<?xml version="1.0"?>
<!DOCTYPE rdf:RDF [
    <!ENTITY dct "http://purl.org/dc/terms/" >
    <!ENTITY foaf "http://xmlns.com/foaf/0.1/" >
    <!ENTITY dcat "http://www.w3.org/ns/dcat#" >
    <!ENTITY owl "http://www.w3.org/2002/07/owl#" >
    <!ENTITY vcard "http://www.w3.org/2006/vcard/ns#" >
    <!ENTITY xsd "http://www.w3.org/2001/XMLSchema#http://www.w3.org/2001/XMLSchema#" >
    <!ENTITY voaf "http://purl.org/vocommons/voaf#" >
    <!ENTITY skos "http://www.w3.org/2004/02/skos/core#" >
    <!ENTITY rdfs "http://www.w3.org/2000/01/rdf-schema#" >
    <!ENTITY rdf "http://www.w3.org/1999/02/22-rdf-syntax-ns#" >
	<!ENTITY cc "http://creativecommons.org/ns#" >
	<!ENTITY vann "http://purl.org/vocab/vann/" >
    <!ENTITY documentation "https://stelar-project.eu/">
    <!ENTITY documentationTitle "DCAT Application Profile for Data Assets in the KLMS Data Catalog">
    <!ENTITY methodology "https://stelar-project.eu/">
    <!ENTITY methodologyTitle "Methodology for Developing the KLMS Data Catalog">
]>
<!-- About the application profile -->
<rdf:RDF xmlns="http://stelar-project.eu/klms#"
     xml:base="http://stelar-project.eu/klms"
	 xmlns:klms="http://stelar-project.eu/klms"
	 xmlns:dcat="http://www.w3.org/ns/dcat#"
	 xmlns:foaf="http://xmlns.com/foaf/0.1/"
     xmlns:rdf="http://www.w3.org/1999/02/22-rdf-syntax-ns#"
	 xmlns:rdfs="http://www.w3.org/2000/01/rdf-schema#"
     xmlns:dct="http://purl.org/dc/terms/"
     xmlns:owl="http://www.w3.org/2002/07/owl#"
     xmlns:xml="http://www.w3.org/XML/1998/namespace"
     xmlns:vcard="http://www.w3.org/2006/vcard/ns#"
     xmlns:xsd="http://www.w3.org/2001/XMLSchema#"
     xmlns:skos="http://www.w3.org/2004/02/skos/core#"
	 xmlns:prov="http://www.w3.org/ns/prov#"
	 xmlns:schema="http://schema.org/"
	 xmlns:vann="http://purl.org/vocab/vann/"
	 xmlns:adms="http://www.w3.org/ns/adms#"
	 xmlns:cc="http://creativecommons.org/ns#"
	 xmlns:time="http://www.w3.org/2006/time#"
	 xmlns:locn="http://www.w3.org/ns/locn#"
	 xmlns:geo="http://www.opengis.net/ont/geosparql#"
	 xmlns:odrl="http://www.w3.org/ns/odrl/2/"
	 xmlns:dc="http://purl.org/dc/elements/1.1/"
	 xmlns:org="http://www.w3.org/ns/org#">
    <owl:Ontology rdf:about="http://stelar-project.eu/klms">
       <owl:imports rdf:resource="https://www.w3.org/ns/dcat"/>
		<rdfs:label xml:lang="en">KLMS model</rdfs:label>
		<dct:title xml:lang="en">Model of Assets in Knowledge Lake Management System (KLMS)</dct:title>
        <rdfs:comment>Ontology of assets (datasets, workflows, users) in Knowledge Lake Management System (KLMS).</rdfs:comment>
		<dct:created rdf:datatype="xsd:date">2023-03-01</dct:created>
		<dct:modified rdf:datatype="xsd:date">2023-10-17</dct:modified>
        <dct:abstract xml:lang="en">This model is used for describing assets in Knowledge Lake Management System (KLMS) based on the Data Catalogue vocabulary (DCAT).</dct:abstract>
        <cc:attributionName xml:lang="en">STELAR project</cc:attributionName>
		<vann:preferredNamespacePrefix>klms</vann:preferredNamespacePrefix>
		<vann:preferredNamespaceUri rdf:resource="http://stelar-project.eu/klms#"/>
        <owl:versionInfo xml:lang="en">0.1</owl:versionInfo>
		<dct:license>
          <rdf:Description rdf:about="https://www.apache.org/licenses/LICENSE-2.0">
            <dct:title>Apache License 2.0</dct:title>
            <cc:attributionName>STELAR project</cc:attributionName>
            <cc:attributionURL rdf:resource="https://stelar-project.eu/"/>
          </rdf:Description>
        </dct:license>
		<dct:creator rdf:parseType="Resource">
          <rdfs:seeAlso rdf:resource="http://web.imis.athena-innovation.gr/~dskoutas/"/>
          <foaf:name>Dimitrios Skoutas</foaf:name>
          <foaf:homepage rdf:resource="http://web.imis.athena-innovation.gr/~dskoutas/"/>
          <schema:affiliation rdf:parseType="Resource">
            <foaf:name>IMSI, Athena Research Center</foaf:name>
            <foaf:homepage rdf:resource="https://www.imsi.athenarc.gr/"/>
          </schema:affiliation>	           
        </dct:creator>
		<dct:creator rdf:parseType="Resource">
          <rdfs:seeAlso rdf:resource="https://www.imsi.athenarc.gr/en/people/member/88"/>
          <foaf:name>Georgios Chatzigeorgakidis</foaf:name>
          <foaf:homepage rdf:resource="https://www.linkedin.com/in/georgios-chatzigeorgakidis-58862759/"/>
          <schema:affiliation rdf:parseType="Resource">
            <foaf:name>IMSI, Athena Research Center</foaf:name>
            <foaf:homepage rdf:resource="https://www.imsi.athenarc.gr/"/>
          </schema:affiliation>	           
        </dct:creator>
		<dct:creator rdf:parseType="Resource">
          <rdfs:seeAlso rdf:resource="https://www.imsi.athenarc.gr/en/people/member/76"/>
          <foaf:name>Kostas Patroumpas</foaf:name>
          <foaf:homepage rdf:resource="https://www.imsi.athenarc.gr/en/people/member/76"/>
          <schema:affiliation rdf:parseType="Resource">
            <foaf:name>IMSI, Athena Research Center</foaf:name>
            <foaf:homepage rdf:resource="https://www.imsi.athenarc.gr/"/>
          </schema:affiliation>	           
        </dct:creator>
		<dct:creator rdf:parseType="Resource">
		 <rdfs:seeAlso rdf:resource="https://www.imsi.athenarc.gr/en/people/member/130"/>
          <foaf:name>Alexandros Zeakis</foaf:name>
          <foaf:homepage rdf:resource="https://www.imsi.athenarc.gr/en/people/member/130"/>     
          <schema:affiliation rdf:parseType="Resource">
            <foaf:name>IMSI, Athena Research Center</foaf:name>
            <foaf:homepage rdf:resource="https://www.imsi.athenarc.gr/"/>
          </schema:affiliation>	  		  
        </dct:creator>
		<dct:creator rdf:parseType="Resource">
		 <rdfs:seeAlso rdf:resource="https://www.imsi.athenarc.gr/en/people/member/132"/>
          <foaf:name>Panos Bethavas</foaf:name>
          <foaf:homepage rdf:resource="https://www.imsi.athenarc.gr/en/people/member/132"/>     
          <schema:affiliation rdf:parseType="Resource">
            <foaf:name>IMSI, Athena Research Center</foaf:name>
            <foaf:homepage rdf:resource="https://www.imsi.athenarc.gr/"/>
          </schema:affiliation>	  		  
        </dct:creator>
    </owl:Ontology>
    



    <!-- 
    ///////////////////////////////////////////////////////////////////////////////////////
    //
    // Datatypes
    //
    ///////////////////////////////////////////////////////////////////////////////////////
     -->


    <!-- http://stelar-project.eu/klms#AccessRightsEnum -->

    <rdfs:Datatype rdf:about="http://stelar-project.eu/klms#AccessRightsEnum">
        <rdfs:comment xml:lang="en">Enumeration of access rights for a Dataset.</rdfs:comment>
        <owl:equivalentClass>
            <rdfs:Datatype>
                <owl:oneOf>
                    <rdf:Description>
                        <rdf:type rdf:resource="http://www.w3.org/1999/02/22-rdf-syntax-ns#List"/>
                        <rdf:first>public</rdf:first>
                        <rdf:rest>
                            <rdf:Description>
                                <rdf:type rdf:resource="http://www.w3.org/1999/02/22-rdf-syntax-ns#List"/>
                                <rdf:first>restricted</rdf:first>
                                <rdf:rest>
                                    <rdf:Description>
                                        <rdf:type rdf:resource="http://www.w3.org/1999/02/22-rdf-syntax-ns#List"/>
                                        <rdf:first>private</rdf:first>
                                        <rdf:rest rdf:resource="http://www.w3.org/1999/02/22-rdf-syntax-ns#nil"/>
                                    </rdf:Description>
                                </rdf:rest>
                            </rdf:Description>
                        </rdf:rest>
                    </rdf:Description>
                </owl:oneOf>
            </rdfs:Datatype>
        </owl:equivalentClass>
    </rdfs:Datatype>
	

    <!-- http://stelar-project.eu/klms#UserRolesEnum -->

    <rdfs:Datatype rdf:about="http://stelar-project.eu/klms#UserRolesEnum">
        <rdfs:comment xml:lang="en">Enumeration of possible roles for a User in an Organization. NOTE: Currently according to CKAN.</rdfs:comment>
        <owl:equivalentClass>
            <rdfs:Datatype>
                <owl:oneOf>
                    <rdf:Description>
                        <rdf:type rdf:resource="http://www.w3.org/1999/02/22-rdf-syntax-ns#List"/>
                        <rdf:first>admin</rdf:first>
                        <rdf:rest>
                            <rdf:Description>
                                <rdf:type rdf:resource="http://www.w3.org/1999/02/22-rdf-syntax-ns#List"/>
                                <rdf:first>editor</rdf:first>
                                <rdf:rest>
                                    <rdf:Description>
                                        <rdf:type rdf:resource="http://www.w3.org/1999/02/22-rdf-syntax-ns#List"/>
                                        <rdf:first>member</rdf:first>
                                        <rdf:rest rdf:resource="http://www.w3.org/1999/02/22-rdf-syntax-ns#nil"/>
                                    </rdf:Description>
                                </rdf:rest>
                            </rdf:Description>
                        </rdf:rest>
                    </rdf:Description>
                </owl:oneOf>
            </rdfs:Datatype>
        </owl:equivalentClass>
    </rdfs:Datatype>
	


<!-- ####################################### -->
<!-- ##===================================## -->
<!-- ##==          PROPERTIES           ==## -->
<!-- ##===================================## --> 
<!-- ####################################### -->

<!--  foaf - name   -->
	<owl:DatatypeProperty rdf:about="http://xmlns.com/foaf/0.1/name">
	  <vann:usageNote xml:lang="en">Recommended property. A name for some thing (e.g., organization, user).</vann:usageNote>
	  <dct:identifier>foaf:name</dct:identifier>
	  <rdfs:domain rdf:resource="http://www.w3.org/2000/01/rdf-schema#Resource"/>
	  <rdfs:range rdf:resource="http://www.w3.org/2000/01/rdf-schema#Literal"/>
	  <rdfs:isDefinedBy rdf:resource="http://xmlns.com/foaf/0.1/"/>
	  <rdfs:comment xml:lang="en">A name for some thing (e.g., organization, user).</rdfs:comment>
	</owl:DatatypeProperty>

<!--  Organization - homepage   -->
	<owl:ObjectProperty rdf:about="http://xmlns.com/foaf/0.1/homepage">
		<vann:usageNote xml:lang="en">Recommended property. A homepage for some thing (e.g., organization, user).</vann:usageNote>
		<dct:identifier>foaf:homepage</dct:identifier>
		<rdfs:subPropertyOf rdf:resource="http://xmlns.com/foaf/0.1/page"/>
		<rdfs:domain rdf:resource="http://stelar-project.eu/klms#Organization"/>
		<rdfs:range rdf:resource="http://xmlns.com/foaf/0.1/Document"/>
		<rdfs:isDefinedBy rdf:resource="http://xmlns.com/foaf/0.1/"/>
		<rdfs:comment xml:lang="en">A homepage for some thing (e.g., organization, user).</rdfs:comment>
	</owl:ObjectProperty>

 <!--  Organization - description  -->
	 <owl:DatatypeProperty rdf:about="http://purl.org/dc/terms/description"> 
		  <vann:usageNote xml:lang="en">Recommended property. This property contains a free-text description of the Organization. This property can be repeated for parallel language versions of the description.</vann:usageNote>
		  <dct:identifier>dct:description</dct:identifier>
		  <rdfs:domain rdf:resource="http://stelar-project.eu/klms#Organization"/>
		  <rdfs:range rdf:resource="http://www.w3.org/2000/01/rdf-schema#Literal"/>
		  <rdfs:label xml:lang="en">Organization - description</rdfs:label>
		  <rdfs:isDefinedBy rdf:resource="http://dublincore.org/documents/dcmi-terms/#terms-description" />
		  <rdfs:comment xml:lang="en">This property contains a free-text description of the Organization. This property can be repeated for parallel language versions of the description.</rdfs:comment>
	 </owl:DatatypeProperty>

<!--  Organization - creation date   -->
	 <owl:DatatypeProperty rdf:about="http://purl.org/dc/terms/created"> 
		  <vann:usageNote xml:lang="en">Recommended property. This property contains the date of formal creation of the Organization.</vann:usageNote>
		  <dct:identifier>dct:created</dct:identifier>
		  <rdfs:domain rdf:resource="http://stelar-project.eu/klms#Organization"/>
		  <rdfs:range rdf:resource="http://www.w3.org/2001/XMLSchema#dateTime"/>
		  <rdfs:label xml:lang="en">Organization - creation date</rdfs:label>
		  <rdfs:isDefinedBy rdf:resource="http://dublincore.org/documents/dcmi-terms/#terms-created" />
		  <rdfs:comment xml:lang="en">This property contains the date of formal creation of the Organization.</rdfs:comment>
	 </owl:DatatypeProperty>
	 
<!--  Organization - logo   -->
	<owl:ObjectProperty rdf:about="http://xmlns.com/foaf/0.1/logo">
		<vann:usageNote xml:lang="en">Optional property. A logo representing some thing (e.g., organization).</vann:usageNote>
		<dct:identifier>foaf:logo</dct:identifier>
		<rdfs:domain rdf:resource="http://stelar-project.eu/klms#Organization"/>
		<rdfs:range rdf:resource="http://www.w3.org/2000/01/rdf-schema#Resource"/>
		<rdfs:isDefinedBy rdf:resource="http://xmlns.com/foaf/0.1/"/>
		<rdfs:comment xml:lang="en">A logo representing some thing (e.g., organization).</rdfs:comment>
	</owl:ObjectProperty>

<!--  User - creation date   -->
	 <owl:DatatypeProperty rdf:about="http://purl.org/dc/terms/created"> 
		  <vann:usageNote xml:lang="en">Recommended property. This property contains the date this User was created.</vann:usageNote>
		  <dct:identifier>dct:created</dct:identifier>
		  <rdfs:domain rdf:resource="http://stelar-project.eu/klms#User"/>
		  <rdfs:range rdf:resource="http://www.w3.org/2001/XMLSchema#dateTime"/>
		  <rdfs:label xml:lang="en">User - creation date</rdfs:label>
		  <rdfs:isDefinedBy rdf:resource="http://dublincore.org/documents/dcmi-terms/#terms-created" />
		  <rdfs:comment xml:lang="en">This property contains the date this User was created.</rdfs:comment>
	 </owl:DatatypeProperty>
	 
<!-- User - accountName -->
	<owl:DatatypeProperty rdf:about="http://xmlns.com/foaf/0.1/accountName">
		<vann:usageNote xml:lang="en">Recommended property. Indicates the name (identifier) associated with a user account.</vann:usageNote>
		<dct:identifier>foaf:accountName</dct:identifier>
		<rdfs:domain rdf:resource="http://stelar-project.eu/klms#User"/>
		<rdfs:range rdf:resource="http://www.w3.org/2000/01/rdf-schema#Literal"/>
		<rdfs:isDefinedBy rdf:resource="http://xmlns.com/foaf/0.1/"/>
		<rdfs:comment xml:lang="en">Indicates the name (identifier) associated with a user account.</rdfs:comment>
	</owl:DatatypeProperty>

 <!--  User - description  -->
	 <owl:DatatypeProperty rdf:about="http://purl.org/dc/terms/description"> 
		  <vann:usageNote xml:lang="en">Recommended property. This property contains a free-text description of the User. This property can be repeated for parallel language versions of the description.</vann:usageNote>
		  <dct:identifier>dct:description</dct:identifier>
		  <rdfs:domain rdf:resource="http://stelar-project.eu/klms#User"/>
		  <rdfs:range rdf:resource="http://www.w3.org/2000/01/rdf-schema#Literal"/>
		  <rdfs:label xml:lang="en">User - description</rdfs:label>
		  <rdfs:isDefinedBy rdf:resource="http://dublincore.org/documents/dcmi-terms/#terms-description" />
		  <rdfs:comment xml:lang="en">This property contains a free-text description of the User. This property can be repeated for parallel language versions of the description.</rdfs:comment>
	 </owl:DatatypeProperty>
	 
<!-- User - mbox -->
	<owl:ObjectProperty rdf:about="http://xmlns.com/foaf/0.1/mbox">
		<vann:usageNote xml:lang="en">Recommended property. A personal mailbox, ie. an Internet mailbox associated with exactly one user.</vann:usageNote>
		<dct:identifier>foaf:mbox</dct:identifier>
		<rdfs:domain rdf:resource="http://stelar-project.eu/klms#User"/>
		<rdfs:range rdf:resource="http://www.w3.org/2000/01/rdf-schema#Resource"/>
		<rdfs:isDefinedBy rdf:resource="http://xmlns.com/foaf/0.1/"/>
		<rdfs:comment xml:lang="en">A personal mailbox, ie. an Internet mailbox associated with exactly one user, the first owner of this mailbox. This is a 'static inverse functional property', in that there is (across time and change) at most one individual that ever has any particular value for foaf:mbox.</rdfs:comment>
	</owl:ObjectProperty>

<!-- User - img -->
	<owl:ObjectProperty rdf:about="http://xmlns.com/foaf/0.1/img">
		<vann:usageNote xml:lang="en">Optional property. An image that can be used to represent a User (e.g., one's photo on a homepage).</vann:usageNote>
		<dct:identifier>foaf:img</dct:identifier>
		<rdf:type rdf:resource="http://www.w3.org/2002/07/owl#ObjectProperty"/>
		<rdfs:domain rdf:resource="http://stelar-project.eu/klms#User"/>
		<rdfs:range rdf:resource="http://xmlns.com/foaf/0.1/Image"/>
		<rdfs:isDefinedBy rdf:resource="http://xmlns.com/foaf/0.1/"/>
		<rdfs:comment xml:lang="en">An image that can be used to represent a User (e.g., one's photo on a homepage).</rdfs:comment>
	</owl:ObjectProperty>

 <!--  User - last active  -->
	 <owl:DatatypeProperty rdf:about="http://stelar-project.eu/klms#lastActive"> 
		  <vann:usageNote xml:lang="en">Recommended property. This property contains the date/time when the User was last logged in the Catalog.</vann:usageNote>
		  <dct:identifier>klms:lastActive</dct:identifier>
		  <rdfs:domain rdf:resource="http://stelar-project.eu/klms#User"/>
		  <rdfs:range rdf:resource="http://www.w3.org/2001/XMLSchema#dateTime"/>
		  <rdfs:label xml:lang="en">User - lastActive</rdfs:label>
		  <rdfs:comment xml:lang="en">This property contains the date/time when the User was last logged in the Catalog.</rdfs:comment>
	 </owl:DatatypeProperty>
	 
<!-- Membership - member -->
	<owl:ObjectProperty rdf:about="http://www.w3.org/ns/org#member">
		<vann:usageNote xml:lang="en">Recommended property. Indicates that a user is involved in a Membership within an Organization.</vann:usageNote>
		<dct:identifier>org:member</dct:identifier>
		<rdfs:domain rdf:resource="http://www.w3.org/ns/org#Membership"/>
		<rdfs:range rdf:resource="http://stelar-project.eu/klms#User"/>
		<rdfs:isDefinedBy rdf:resource="http://www.w3.org/ns/org"/>
		<rdfs:comment xml:lang="en">Indicates that a user is is involved in a Membership within an Organization.</rdfs:comment>
	</owl:ObjectProperty>

<!-- Membership - organization -->
	<owl:ObjectProperty rdf:about="http://www.w3.org/ns/org#organization">
		<vann:usageNote xml:lang="en">Recommended property. Indicates the Organization in which a User is a member.</vann:usageNote>
		<dct:identifier>org:organization</dct:identifier>
		<rdfs:domain rdf:resource="http://www.w3.org/ns/org#Membership"/>
		<rdfs:range rdf:resource="http://stelar-project.eu/klms#Organization"/>
		<rdfs:isDefinedBy rdf:resource="http://www.w3.org/ns/org"/>
		<rdfs:comment xml:lang="en">Indicates the Organization in which a User is a member.</rdfs:comment>
	</owl:ObjectProperty>
	
<!-- Membership - role -->
	<owl:ObjectProperty rdf:about="http://www.w3.org/ns/org#role">
		<vann:usageNote xml:lang="en">Recommended property. Indicates the Role that a User plays in a Membership relationship with an Organization.</vann:usageNote>
		<dct:identifier>org:role</dct:identifier>
		<rdfs:domain rdf:resource="http://www.w3.org/ns/org#Membership"/>
		<rdfs:range rdf:resource="http://www.w3.org/ns/org#Role"/>
		<rdfs:isDefinedBy rdf:resource="http://www.w3.org/ns/org"/>
		<rdfs:comment xml:lang="en">Indicates the Role that a User plays in a Membership relationship with an Organization.</rdfs:comment>
	</owl:ObjectProperty>

	
 <!--  Role - specification  -->
	 <owl:DatatypeProperty rdf:about="http://stelar-project.eu/klms#roleSpecs"> 
		  <vann:usageNote xml:lang="en">Recommended property. This property contains the specification of a User's role (admin, editor, or member) regarding the Catalog within an Organization.</vann:usageNote>
		  <dct:identifier>klms:roleSpecs</dct:identifier>
		  <rdfs:domain rdf:resource="http://www.w3.org/ns/org#Role"/>
		  <rdfs:range rdf:resource="http://stelar-project.eu/klms#UserRolesEnum"/>
		  <rdfs:label xml:lang="en">Role -specification</rdfs:label>
		  <rdfs:comment xml:lang="en">This property contains the specification of a User's role (admin, editor, or member) regarding the Catalog within an Organization.</rdfs:comment>
	 </owl:DatatypeProperty>

	
<!-- ====================================== -->
<!-- ==       DATASET - Properties       == -->
<!-- ====================================== --> 
<!-- ==       Mandatory Properties       == -->
<!-- ====================================== --> 

<!--  Dataset - identifier   -->
	 <owl:DatatypeProperty rdf:about="http://purl.org/dc/terms/identifier"> 
		  <vann:usageNote xml:lang="en">Optional property. This property contains the main identifier for the Dataset, e.g. a UUID or other unique identifier in the context of the Catalogue.</vann:usageNote>
		  <dct:identifier>dct:identifier</dct:identifier>
		  <rdfs:domain rdf:resource="http://www.w3.org/ns/dcat#Dataset"/>
		  <rdfs:range rdf:resource="http://www.w3.org/2000/01/rdf-schema#Literal"/>
		  <rdfs:label xml:lang="en">Dataset - identifier</rdfs:label>
		  <dct:acrualPeriodicity rdf:resource="http://dublincore.org/documents/dcmi-terms/#terms-identifier" />
		  <rdfs:comment xml:lang="en">This property contains the main identifier for the Dataset, e.g. a UUID or other unique identifier in the context of the Catalogue.</rdfs:comment>
	 </owl:DatatypeProperty>
 
 <!--  Dataset - description  -->
	 <owl:DatatypeProperty rdf:about="http://purl.org/dc/terms/description"> 
		  <vann:usageNote xml:lang="en">Mandatory property. This property contains a free-text account of the Dataset. This property can be repeated for parallel language versions of the description.</vann:usageNote>
		  <dct:identifier>dct:description</dct:identifier>
		  <rdfs:domain rdf:resource="http://www.w3.org/ns/dcat#Dataset"/>
		  <rdfs:range rdf:resource="http://www.w3.org/2000/01/rdf-schema#Literal"/>
		  <rdfs:label xml:lang="en">Dataset - description</rdfs:label>
		  <rdfs:isDefinedBy rdf:resource="http://dublincore.org/documents/dcmi-terms/#terms-description" />
		  <rdfs:comment xml:lang="en">This property contains a free-text account of the Dataset. This property can be repeated for parallel language versions of the description.</rdfs:comment>
	 </owl:DatatypeProperty>
 
<!--  Dataset - title  -->
	 <owl:DatatypeProperty rdf:about="http://purl.org/dc/terms/title"> 
		  <vann:usageNote xml:lang="en">Mandatory property. This property contains a name given to the Dataset. This property can be repeated for parallel language versions of the name.</vann:usageNote>
		  <dct:identifier>dct:title</dct:identifier>
		  <rdfs:domain rdf:resource="http://www.w3.org/ns/dcat#Dataset"/>
		  <rdfs:range rdf:resource="http://www.w3.org/2000/01/rdf-schema#Literal"/>
		  <rdfs:label xml:lang="en">Dataset - title</rdfs:label>
		  <rdfs:isDefinedBy rdf:resource="http://dublincore.org/documents/dcmi-terms/#terms-title" />
		  <rdfs:comment xml:lang="en">This property contains a name (title) given to the Dataset. This property can be repeated for parallel language versions of the name.</rdfs:comment>
	 </owl:DatatypeProperty>

<!--  Dataset - keyword/tag  -->
	 <owl:DatatypeProperty rdf:about="http://www.w3.org/ns/dcat#keyword"> 
		  <vann:usageNote xml:lang="en">Recommended property. This property contains a keyword or tag characterizing the Dataset.</vann:usageNote>
		  <dct:identifier>dcat:keyword</dct:identifier>
		  <rdfs:domain rdf:resource="http://www.w3.org/ns/dcat#Dataset"/>
		  <rdfs:range rdf:resource="http://www.w3.org/2001/XMLSchema#string"/>
		  <rdfs:label xml:lang="en">Dataset - keyword/tag</rdfs:label>
		  <rdfs:isDefinedBy rdf:resource="https://www.w3.org/TR/vocab-dcat-2/#Property:resource_keyword" />
		  <rdfs:comment xml:lang="en">This property contains a keyword or tag characterizing the Dataset.</rdfs:comment>
	 </owl:DatatypeProperty>
 
 
<!-- ============================= -->
<!--    Recommended properties     -->
<!-- ============================= -->

<!--  Dataset - distribution  -->
	 <owl:ObjectProperty rdf:about="http://www.w3.org/ns/dcat#distribution"> 
		  <vann:usageNote xml:lang="en">Recommended property. This property links the Dataset to an available Distribution.</vann:usageNote>
		  <dct:identifier>dcat:distribution</dct:identifier>
		  <rdfs:label xml:lang="en">Dataset - distribution</rdfs:label>
		  <rdfs:isDefinedBy rdf:resource="https://www.w3.org/TR/vocab-dcat-2/#Property:dataset_distribution" />
		  <rdfs:comment xml:lang="en">This property links the Dataset to an available Distribution.</rdfs:comment>
	 </owl:ObjectProperty>
 
<!--  Dataset - license   -->
	 <owl:DatatypeProperty rdf:about="http://purl.org/dc/terms/license"> 
		  <vann:usageNote xml:lang="en">Recommended property. This property refers to the license under which the Dataset is made available.</vann:usageNote>
		  <dct:identifier>dct:license</dct:identifier>
		  <rdfs:label xml:lang="en">Dataset - license</rdfs:label>
		  <rdfs:isDefinedBy rdf:resource="http://dublincore.org/documents/dcmi-terms/#terms-license" />
		  <rdfs:comment xml:lang="en">This property refers to the licence under which the Dataset is made available. NOTE: License in KLMS refers to the Dataset (as in CKAN); instead, in the DCAT model it is at the Distribution level.</rdfs:comment>
	 </owl:DatatypeProperty>
 
 <!--  Dataset - theme  -->
	 <owl:ObjectProperty rdf:about="http://www.w3.org/ns/dcat#theme"> 
		  <vann:usageNote xml:lang="en">Recommended property. This property refers to a thematic category of the Dataset. A Dataset may be associated with multiple themes.</vann:usageNote>
		  <dct:identifier>dcat:theme</dct:identifier>
		  <rdfs:label xml:lang="en">Dataset - theme</rdfs:label>
		  <rdfs:isDefinedBy rdf:resource="https://www.w3.org/TR/vocab-dcat-2/#Property:resource_type" />
		  <rdfs:comment xml:lang="en">This property refers to a thematic category of the Dataset. A Dataset may be associated with multiple themes. Subproperty of dct:subject</rdfs:comment>
	 </owl:ObjectProperty>
 
<!--  Dataset - contact point -->
	 <owl:ObjectProperty rdf:about="http://www.w3.org/ns/dcat#contactPoint"> 
		  <vann:usageNote xml:lang="en">Recommended property.This property contains contact information that can be used for sending comments about the Dataset.</vann:usageNote>
		  <dct:identifier>dcat:contactPoint</dct:identifier>
		  <rdfs:label xml:lang="en">Dataset - contact point</rdfs:label>
		  <rdfs:domain rdf:resource="http://www.w3.org/ns/dcat#Dataset"/>
		  <rdfs:range rdf:resource="http://www.w3.org/2006/vcard/ns#Kind"/>
		  <rdfs:isDefinedBy rdf:resource="https://www.w3.org/TR/vocab-dcat-2/#Property:resource_contact_point" />
		  <rdfs:comment xml:lang="en">This property contains contact information that can be used for sending comments about the Dataset.</rdfs:comment>
	 </owl:ObjectProperty>
 
<!--  Dataset - publisher  -->
	 <owl:ObjectProperty rdf:about="http://purl.org/dc/terms/publisher"> 
		  <vann:usageNote xml:lang="en">Recommended property. This property refers to an entity (organisation) responsible for making the Dataset available.</vann:usageNote>
		  <dct:identifier>dct:publisher</dct:identifier>
		  <rdfs:domain rdf:resource="http://www.w3.org/ns/dcat#Dataset"/>
		  <rdfs:range rdf:resource="http://xmlns.com/foaf/0.1/Organization"/>
		  <rdfs:label xml:lang="en">Dataset - publisher</rdfs:label>
		  <rdfs:isDefinedBy rdf:resource="http://dublincore.org/documents/dcmi-terms/#terms-publisher" />
		  <rdfs:comment xml:lang="en">This property refers to an entity (organisation) responsible for making the Dataset available.</rdfs:comment>
	 </owl:ObjectProperty>
 
<!--  Dataset - spatial/geographical coverage   -->
	 <owl:ObjectProperty rdf:about="http://purl.org/dc/terms/spatial"> 
		  <vann:usageNote xml:lang="en">Recommended property. This property refers to a geographic region that is covered by the Dataset. </vann:usageNote>
		  <dct:identifier>dct:spatial</dct:identifier>
		  <rdfs:domain rdf:resource="http://www.w3.org/ns/dcat#Dataset"/>
		  <rdfs:range rdf:resource="http://purl.org/dc/terms/Location"/>
		  <rdfs:label xml:lang="en">Dataset - spatial/ geographical coverage</rdfs:label>
		  <rdfs:isDefinedBy rdf:resource="http://dublincore.org/documents/dcmi-terms/#terms-spatial" />
		  <rdfs:comment xml:lang="en">This property refers to a geographic region that is covered by the Dataset.</rdfs:comment>
	 </owl:ObjectProperty>

 <!--  Dataset - temporal coverage   -->
	 <owl:ObjectProperty rdf:about="http://purl.org/dc/terms/temporal"> 
		  <vann:usageNote xml:lang="en">Recommended property. This property refers to a temporal period that the Dataset covers.</vann:usageNote>
		  <dct:identifier>dct:temporal</dct:identifier>
		  <rdfs:domain rdf:resource="http://www.w3.org/ns/dcat#Dataset"/>
		  <rdfs:range rdf:resource="http://purl.org/dc/terms/PeriodOfTime"/>
		  <rdfs:label xml:lang="en">Dataset - temporal coverage</rdfs:label>
		  <rdfs:isDefinedBy rdf:resource="http://dublincore.org/documents/dcmi-terms/#terms-temporal" />
		  <rdfs:comment xml:lang="en">This property refers to a temporal period that the Dataset covers.</rdfs:comment>
	 </owl:ObjectProperty>

<!-- ====================================== --> 
<!--         Optional properties            -->
<!-- ====================================== --> 

<!--  Dataset - type   -->
	 <owl:DatatypeProperty rdf:about="http://purl.org/dc/terms/type"> 
		  <vann:usageNote xml:lang="en">Optional property. This property refers to the type of the Dataset. NOTE: A controlled vocabulary for the values has not been established.</vann:usageNote>
		  <dct:identifier>dct:type</dct:identifier>
		  <rdfs:label xml:lang="en">Dataset - type </rdfs:label>
		  <rdfs:isDefinedBy rdf:resource="http://dublincore.org/documents/dcmi-terms/#terms-type" />
		  <rdfs:comment xml:lang="en">This property refers to the type of the Dataset. NOTE: A controlled vocabulary for the values has not been established.</rdfs:comment>
	 </owl:DatatypeProperty> 
 
<!--  Dataset - conforms to  -->
	 <owl:ObjectProperty rdf:about="http://purl.org/dc/terms/conformsTo"> 
		  <vann:usageNote xml:lang="en">Optional property. This property refers to an implementing rule, standard, or other specification.</vann:usageNote>
		  <dct:identifier>dct:conformsTo</dct:identifier>
		  <rdfs:domain rdf:resource="http://www.w3.org/ns/dcat#Dataset"/>
		  <rdfs:range rdf:resource="http://purl.org/dc/terms/Standard"/>
		  <rdfs:label xml:lang="en">Dataset - conforms to</rdfs:label>
		  <rdfs:isDefinedBy rdf:resource="http://dublincore.org/documents/dcmi-terms/#terms-conformsTo" />
		  <rdfs:comment xml:lang="en">This property refers to an implementing rule, standard, or other specification.</rdfs:comment>
	 </owl:ObjectProperty>
 
<!--  Dataset - update frequency   -->
	 <owl:ObjectProperty rdf:about="http://purl.org/dc/terms/accrualPeriodicity"> 
		  <vann:usageNote xml:lang="en">Optional property. This property refers to the frequency at which Dataset is updated.</vann:usageNote>
		  <dct:identifier>dct:accrualPeriodicity</dct:identifier>
		  <rdfs:domain rdf:resource="http://www.w3.org/ns/dcat#Dataset"/>
		  <rdfs:range rdf:resource="http://purl.org/dc/terms/Frequency"/>
		  <rdfs:label xml:lang="en">Dataset - update frequency</rdfs:label>
		  <rdfs:isDefinedBy rdf:resource="http://dublincore.org/documents/dcmi-terms/#terms-accrualPeriodicity" />
		  <rdfs:comment xml:lang="en">This property refers to the frequency at which Dataset is updated.</rdfs:comment>
	 </owl:ObjectProperty>
 
<!--  Dataset - landing page   -->
	 <owl:ObjectProperty rdf:about="http://www.w3.org/ns/dcat#landingPage"> 
		  <vann:usageNote xml:lang="en">Optional property. This property refers to a web page that provides access to the Dataset, its Distributions and/or additional information. </vann:usageNote>
		  <dct:identifier>dcat:landingPage</dct:identifier>
		  <rdfs:domain rdf:resource="http://www.w3.org/ns/dcat#Dataset"/>
		  <rdfs:range rdf:resource="http://xmlns.com/foaf/0.1/Document"/>
		  <rdfs:label xml:lang="en">Dataset - landing page</rdfs:label>
		  <rdfs:isDefinedBy rdf:resource="https://www.w3.org/TR/vocab-dcat-2/#Property:resource_landing_page" />
		  <rdfs:comment xml:lang="en">This property refers to a web page that provides access to the Dataset, its Distributions and/or additional information.</rdfs:comment>
	 </owl:ObjectProperty>
 
<!--  Dataset - language   -->
	 <owl:ObjectProperty rdf:about="http://purl.org/dc/terms/language"> 
		  <vann:usageNote xml:lang="en">Optional property. This property refers to a language of the Dataset. This property can be repeated if there are multiple languages in the Dataset.</vann:usageNote>
		  <dct:identifier>dct:language</dct:identifier>
		  <rdfs:domain rdf:resource="http://www.w3.org/ns/dcat#Dataset"/>
		  <rdfs:range rdf:resource="http://purl.org/dc/terms/LinguisticSystem"/>
		  <rdfs:label xml:lang="en">Dataset - language</rdfs:label>
		  <rdfs:isDefinedBy rdf:resource="http://dublincore.org/documents/dcmi-terms/#terms-language" />
		  <rdfs:comment xml:lang="en">This property refers to a language of the Dataset. This property can be repeated if there are multiple languages in the Dataset.</rdfs:comment>
	 </owl:ObjectProperty>
 
<!--  Dataset - release date   -->
	 <owl:DatatypeProperty rdf:about="http://purl.org/dc/terms/issued"> 
		  <vann:usageNote xml:lang="en">Optional property. This property contains the date of formal issuance (e.g., publication) of the Dataset.</vann:usageNote>
		  <dct:identifier>dct:issued</dct:identifier>
		  <rdfs:domain rdf:resource="http://www.w3.org/ns/dcat#Dataset"/>
		  <rdfs:range rdf:resource="http://www.w3.org/2001/XMLSchema#dateTime"/>
		  <rdfs:label xml:lang="en">Dataset - release date</rdfs:label>
		  <rdfs:isDefinedBy rdf:resource="http://dublincore.org/documents/dcmi-terms/#terms-issued" />
		  <rdfs:comment xml:lang="en">This property contains the date of formal issuance (e.g., publication) of the Dataset.</rdfs:comment>
	 </owl:DatatypeProperty>
 
<!--  Dataset - update/modification date   -->
	 <owl:DatatypeProperty rdf:about="http://purl.org/dc/terms/modified"> 
		  <vann:usageNote xml:lang="en">Optional property. This property contains the most recent date on which the Dataset was changed or modified.</vann:usageNote>
		  <dct:identifier>dct:modified</dct:identifier>
		  <rdfs:domain rdf:resource="http://www.w3.org/ns/dcat#Dataset"/>
		  <rdfs:range rdf:resource="http://www.w3.org/2001/XMLSchema#dateTime"/>
		  <rdfs:label xml:lang="en">Dataset - update/ modification date</rdfs:label>
		  <rdfs:isDefinedBy rdf:resource="http://dublincore.org/documents/dcmi-terms/#terms-modified" />
		  <rdfs:comment xml:lang="en">This property contains the most recent date on which the Dataset was changed or modified.</rdfs:comment>
	 </owl:DatatypeProperty>
 
 <!--  Dataset - temporal resolution -->
 <!--
	 <owl:DatatypeProperty rdf:about="http://www.w3.org/ns/dcat#temporalResolution"> 
	  <vann:usageNote xml:lang="en">Optional property. This property refers to the minimum time period resolvable in the dataset. </vann:usageNote>
	  <dct:identifier>dcat:temporalResolution</dct:identifier>
	  <rdfs:label xml:lang="en">Dataset - temporal resolution </rdfs:label>
	  <rdfs:domain rdf:resource="http://www.w3.org/ns/dcat#Dataset"/>
	  <rdfs:range rdf:resource="http://www.w3.org/2001/XMLSchema#duration"/>
	  <rdfs:isDefinedBy rdf:resource="https://www.w3.org/TR/vocab-dcat-2/#Property:dataset_temporal_resolution" />
	  <rdfs:comment xml:lang="en">This property refers to the minimum time period resolvable in the dataset. If the dataset is a time-series this should correspond to the spacing of items in the series. For other kinds of dataset, this property will usually indicate the smallest time difference between items in the dataset.</rdfs:comment>
	 </owl:DatatypeProperty>
 -->
 
 <!--  Dataset - spatial resolution -->
 <!--
	 <owl:DatatypeProperty rdf:about="http://www.w3.org/ns/dcat#spatialResolutionInMeters"> 
	  <vann:usageNote xml:lang="en">Optional property. This property refers to the minimum spatial separation resolvable in a dataset, measured in meters. </vann:usageNote>
	  <dct:identifier>dcat:spatialResolutionInMeters</dct:identifier>
	  <rdfs:label xml:lang="en">Dataset - spatial resolution</rdfs:label>
	  <rdfs:domain rdf:resource="http://www.w3.org/ns/dcat#Dataset"/>
	  <rdfs:range rdf:resource="http://www.w3.org/2001/XMLSchema#decimal"/>
	  <rdfs:isDefinedBy rdf:resource="https://www.w3.org/TR/vocab-dcat-2/#Property:dataset_spatial_resolution" />
	  <rdfs:comment xml:lang="en">This property refers to the  minimum spatial separation resolvable in a dataset, measured in meters.</rdfs:comment>
	 </owl:DatatypeProperty>
-->

<!--  Dataset - documentation -->
	 <owl:ObjectProperty rdf:about="http://xmlns.com/foaf/0.1/page"> 
		  <vann:usageNote xml:lang="en">Optional property. This property refers to a page or document about this Dataset.</vann:usageNote>
		  <dct:identifier>foaf:page</dct:identifier>
		  <rdfs:domain rdf:resource="http://www.w3.org/ns/dcat#Dataset"/>
		  <rdfs:range rdf:resource="http://xmlns.com/foaf/0.1/Document"/>
		  <rdfs:label xml:lang="en">Dataset - documentation</rdfs:label>
		  <rdfs:isDefinedBy rdf:resource="http://xmlns.com/foaf/spec/#term_page" />
		  <rdfs:comment xml:lang="en">This property refers to a page or document about this Dataset.</rdfs:comment>
	 </owl:ObjectProperty>

<!--  Dataset - access rights   -->
	 <owl:DatatypeProperty rdf:about="http://purl.org/dc/terms/accessRights"> 
		  <vann:usageNote xml:lang="en">Optional property. This property refers to information that indicates whether the Dataset is open data, has access restrictions or is not public. A controlled vocabulary with three members (:public, :restricted, :private) has been created.</vann:usageNote>
		  <dct:identifier>dct:accessRights</dct:identifier>
		  <rdfs:domain rdf:resource="http://www.w3.org/ns/dcat#Dataset"/>
		  <rdfs:range rdf:resource="http://stelar-project.eu/klms#AccessRightsEnum"/>
		  <rdfs:label xml:lang="en">Dataset - access Rights</rdfs:label>
		  <rdfs:isDefinedBy rdf:resource="http://dublincore.org/documents/dcmi-terms/#terms-accessRights" />
		  <rdfs:comment xml:lang="en">This property refers to information that indicates whether the Dataset is open data, has access restrictions or is not public. A controlled vocabulary with three members (:public, :restricted, :private) has been created.</rdfs:comment>
	 </owl:DatatypeProperty>
 
 <!--  Dataset - creator  -->
	 <owl:ObjectProperty rdf:about="http://purl.org/dc/terms/creator"> 
		  <vann:usageNote xml:lang="en">Optional property. This property refers to the person primarily responsible for creating the resource.</vann:usageNote>
		  <dct:identifier>dct:creator</dct:identifier>
		  <rdfs:domain rdf:resource="http://www.w3.org/ns/dcat#Dataset"/>
		  <rdfs:range rdf:resource="http://stelar-project.eu/klms#User"/>
		  <rdfs:label xml:lang="en">Dataset - creator</rdfs:label>
		  <rdfs:isDefinedBy rdf:resource="https://www.dublincore.org/specifications/dublin-core/dcmi-terms/#terms-creator" />
		  <rdfs:comment xml:lang="en">This property refers to the person primarily responsible for creating the resource.</rdfs:comment>
	 </owl:ObjectProperty>	 
	 
 <!--  Dataset - version   -->
	 <owl:AnnotationProperty rdf:about="http://www.w3.org/2002/07/owl#versionInfo"> 
		  <vann:usageNote xml:lang="en">Optional property. This property contains a version number or other version designation of the Dataset.</vann:usageNote>
		  <dct:identifier>owl:versionInfo</dct:identifier>
		  <rdfs:domain rdf:resource="http://www.w3.org/ns/dcat#Dataset"/>
		  <rdfs:label xml:lang="en">Dataset - version</rdfs:label>
		  <rdfs:isDefinedBy rdf:resource="http://www.w3.org/2002/07/owl#" />
		  <rdfs:comment xml:lang="en">This property contains a version number or other version designation of the Dataset.</rdfs:comment>
	 </owl:AnnotationProperty>
 
<!--  Dataset - version notes   -->
	 <owl:DatatypeProperty rdf:about="http://www.w3.org/ns/adms#versionNotes"> 
		  <vann:usageNote xml:lang="en">Optional property. This property contains a description of the differences between this version and a previous version of the Dataset.</vann:usageNote>
		  <dct:identifier>adms:versionNotes</dct:identifier>
		  <rdfs:domain rdf:resource="http://www.w3.org/ns/dcat#Dataset"/>
		  <rdfs:label xml:lang="en">Dataset - version notes</rdfs:label>
		  <rdfs:isDefinedBy rdf:resource="https://www.w3.org/TR/vocab-adms/#adms-versionnotes" />
		  <rdfs:comment xml:lang="en">This property contains a description of the differences between this version and a previous version of the Dataset.</rdfs:comment>
	 </owl:DatatypeProperty>

 <!--  Dataset - is Version Of   -->
	 <owl:ObjectProperty rdf:about="http://purl.org/dc/terms/isVersionOf"> 
		  <vann:usageNote xml:lang="en">Optional property. This property refers to a related Dataset of which the described Dataset is a version, edition, or adaptation.</vann:usageNote>
		  <dct:identifier>dct:isVersionOf</dct:identifier>
		  <rdfs:domain rdf:resource="http://www.w3.org/ns/dcat#Dataset"/>
		  <rdfs:label xml:lang="en">Dataset - is Version Of</rdfs:label>
		  <rdfs:isDefinedBy rdf:resource="http://dublincore.org/documents/dcmi-terms/#terms-isVersionOf" />
		  <rdfs:comment xml:lang="en">This property refers to a related Dataset of which the described Dataset is a version, edition, or adaptation.</rdfs:comment>
	 </owl:ObjectProperty> 
 
  <!--  Dataset - has Version   -->
	 <owl:ObjectProperty rdf:about="http://purl.org/dc/terms/hasVersion"> 
		  <vann:usageNote xml:lang="en">Optional property.This property refers to a related Dataset that is a version, edition, or adaptation of the described Dataset.</vann:usageNote>
		  <dct:identifier>dct:hasVersion</dct:identifier>
		  <rdfs:domain rdf:resource="http://www.w3.org/ns/dcat#Dataset"/>
		  <rdfs:label xml:lang="en">Dataset - has Version</rdfs:label>
		  <rdfs:isDefinedBy rdf:resource="http://dublincore.org/documents/dcmi-terms/#terms-hasVersion" />
		  <rdfs:comment xml:lang="en">This property refers to a related Dataset that is a version, edition, or adaptation of the described Dataset.</rdfs:comment>
	 </owl:ObjectProperty> 
 
 <!--  Dataset - provenance   -->
	 <owl:ObjectProperty rdf:about="http://purl.org/dc/terms/provenance"> 
		  <vann:usageNote xml:lang="en">Optional property. This property contains a statement about the lineage of a Dataset.</vann:usageNote>
		  <dct:identifier>dct:provenance</dct:identifier>
		  <rdfs:domain rdf:resource="http://www.w3.org/ns/dcat#Dataset"/>
		  <rdfs:label xml:lang="en">Dataset - provenance</rdfs:label>
		  <rdfs:isDefinedBy rdf:resource="http://dublincore.org/documents/dcmi-terms/#terms-provenance" />
		  <rdfs:comment xml:lang="en">This property contains a statement about the lineage of a Dataset.</rdfs:comment>
	 </owl:ObjectProperty> 
 
<!--  Dataset - alternate identifier   -->
	 <owl:ObjectProperty rdf:about="http://www.w3.org/ns/adms#identifier"> 
		  <vann:usageNote xml:lang="en">Optional property. This property refers to a secondary identifier of the Dataset, such as MAST/ADS[1], DataCite[2], DOI[3], EZID[4] or W3ID[5].</vann:usageNote>
		  <dct:identifier>adms:identifier</dct:identifier>
		  <rdfs:domain rdf:resource="http://www.w3.org/ns/dcat#Dataset"/>
		  <rdfs:label xml:lang="en">Dataset - alternate identifier</rdfs:label>
		  <rdfs:isDefinedBy rdf:resource="https://www.w3.org/TR/vocab-adms/#adms-identifier" />
		  <rdfs:comment xml:lang="en">This property refers to a secondary identifier of the Dataset, such as MAST/ADS[1], DataCite[2], DOI[3], EZID[4] or W3ID[5].</rdfs:comment>
	 </owl:ObjectProperty>

 
<!-- ====================================== --> 
<!-- ==   Location - Properties    == --> 
<!-- ====================================== --> 

<!--  Location - geometry  -->
	 <owl:DatatypeProperty rdf:about="http://www.w3.org/ns/locn#geometry"> 
		  <vann:usageNote xml:lang="en">Optional property. This property associates a resource with its corresponding geometry.</vann:usageNote>
		  <dct:identifier>locn:geometry </dct:identifier>
		  <rdfs:domain rdf:resource="http://purl.org/dc/terms/Location"/>
		  <rdfs:range rdf:resource="http://www.w3.org/2000/01/rdf-schema#Literal"/>
		  <rdfs:label xml:lang="en">Location - geometry</rdfs:label>
		  <rdfs:isDefinedBy rdf:resource= "https://www.w3.org/TR/vocab-dcat-2/#Property:location_geometry" /> 
		  <rdfs:comment xml:lang="en">This property associates a resource with its corresponding geometry.</rdfs:comment>
	 </owl:DatatypeProperty>

 <!--  Location-  bounding box  -->
	 <owl:DatatypeProperty rdf:about="http://www.w3.org/ns/dcat#bbox"> 
		  <vann:usageNote xml:lang="en">Recommended property. This propert refers to the geographic bounding box of a resource.</vann:usageNote>
		  <dct:identifier> dcat:bbox</dct:identifier>
		  <rdfs:domain rdf:resource="http://purl.org/dc/terms/Location"/>
		  <rdfs:range rdf:resource="http://www.w3.org/2000/01/rdf-schema#Literal"/>
		  <rdfs:label xml:lang="en">Location - bounding box </rdfs:label>
		  <rdfs:isDefinedBy rdf:resource= "https://www.w3.org/TR/vocab-dcat-2/#Property:location_bbox" />
		  <rdfs:comment xml:lang="en">This propert refers to the geographic bounding box of a resource.</rdfs:comment>
	 </owl:DatatypeProperty>

 <!--  Location- centroid  -->
	 <owl:DatatypeProperty rdf:about="http://www.w3.org/ns/dcat#centroid"> 
		  <vann:usageNote xml:lang="en">Recommended property. This property refers to the geographic center (centroid) of a resource.</vann:usageNote>
		  <dct:identifier>dcat:centroid</dct:identifier>
		  <rdfs:domain rdf:resource="http://purl.org/dc/terms/Location"/>
		  <rdfs:range rdf:resource="http://www.w3.org/2000/01/rdf-schema#Literal"/>
		  <rdfs:label xml:lang="en">Location - centroid</rdfs:label>
		  <rdfs:isDefinedBy rdf:resource= "https://www.w3.org/TR/vocab-dcat-2/#Property:location_centroid" /> 
		  <rdfs:comment xml:lang="en">This property refers to the geographic center (centroid) of a resource</rdfs:comment>
	 </owl:DatatypeProperty>

<!-- ====================================== --> 
<!-- ==   Period Of Time - Properties    == --> 
<!-- ====================================== --> 

<!--  Period Of Time - start date  -->
	 <owl:DatatypeProperty rdf:about="http://www.w3.org/ns/dcat#startDate"> 
		  <vann:usageNote xml:lang="en">Recommended property. This property contains the start of the period.</vann:usageNote>
		  <dct:identifier>dcat:startDate</dct:identifier>
		  <rdfs:domain rdf:resource="http://purl.org/dc/terms/PeriodOfTime"/>
		  <rdfs:range rdf:resource="http://www.w3.org/2001/XMLSchema#dateTime"/>
		  <rdfs:label xml:lang="en">Period Of Time - start date</rdfs:label>
		  <rdfs:isDefinedBy rdf:resource="https://www.w3.org/TR/vocab-dcat-2/#Property:period_start_date" />
	  <rdfs:comment xml:lang="en">This property contains the start of the period.</rdfs:comment>
	 </owl:DatatypeProperty>
 
<!--  Period Of Time - end date  -->
	 <owl:DatatypeProperty rdf:about="http://www.w3.org/ns/dcat#endDate"> 
		  <vann:usageNote xml:lang="en">Recommended property. This property contains the end of the period.</vann:usageNote>
		  <dct:identifier>dcat:endDate</dct:identifier>
		  <rdfs:domain rdf:resource="http://purl.org/dc/terms/PeriodOfTime"/>
		  <rdfs:range rdf:resource="http://www.w3.org/2001/XMLSchema#dateTime"/>
		  <rdfs:label xml:lang="en">Period Of Time - end date</rdfs:label>
		  <rdfs:isDefinedBy rdf:resource="https://www.w3.org/TR/vocab-dcat-2/#Property:period_end_date" />
		  <rdfs:comment xml:lang="en">This property contains the end of the period.</rdfs:comment>
	 </owl:DatatypeProperty>

<!-- ====================================== --> 
<!-- ==   KeyValuePair - Properties    == --> 
<!-- ====================================== --> 

	 <owl:DatatypeProperty rdf:about="http://stelar-project.eu/klms#key"> 
		  <vann:usageNote xml:lang="en">Recommended property. This property contains the key of a KeyValuePair.</vann:usageNote>
		  <dct:identifier>klms:key</dct:identifier>
		  <rdfs:domain rdf:resource="http://stelar-project.eu/klms#KeyValuePair"/>
		  <rdfs:range rdf:resource="http://www.w3.org/2001/XMLSchema#string"/>
		  <rdfs:label xml:lang="en">KeyValuePair - key</rdfs:label>
		  <rdfs:comment xml:lang="en">This property contains the key of a KeyValuePair.</rdfs:comment>
	 </owl:DatatypeProperty>
	 
	<owl:DatatypeProperty rdf:about="http://stelar-project.eu/klms#value"> 
		  <vann:usageNote xml:lang="en">Recommended property. This property contains the value of a KeyValuePair.</vann:usageNote>
		  <dct:identifier>klms:value</dct:identifier>
		  <rdfs:domain rdf:resource="http://stelar-project.eu/klms#KeyValuePair"/>
		  <rdfs:range rdf:resource="http://www.w3.org/2001/XMLSchema#string"/>
		  <rdfs:label xml:lang="en">KeyValuePair - value</rdfs:label>
		  <rdfs:comment xml:lang="en">This property contains the value of a KeyValuePair.</rdfs:comment>
	 </owl:DatatypeProperty> 
	

<!-- ====================================== --> 
<!-- ==   Category - Properties    == --> 
<!-- ====================================== --> 

	 <owl:DatatypeProperty rdf:about="http://stelar-project.eu/klms#name"> 
		  <vann:usageNote xml:lang="en">Optional property. The name (title or type) of a class representing a category in a categorical distribution.</vann:usageNote>
		  <dct:identifier>klms:name</dct:identifier>
		  <rdfs:domain rdf:resource="http://stelar-project.eu/klms#Category"/>
		  <rdfs:range rdf:resource="http://www.w3.org/2001/XMLSchema#string"/>
		  <rdfs:label xml:lang="en">Category - name</rdfs:label>
		  <rdfs:comment xml:lang="en">The name (title or type) of a class representing a category in a categorical distribution.</rdfs:comment>
	 </owl:DatatypeProperty>
	 
<!--
	 <owl:DatatypeProperty rdf:about="http://purl.org/dc/terms/title"> 
		  <vann:usageNote xml:lang="en">Optional property. The name (title or type) of a class representing a category in a categorical distribution.</vann:usageNote>
		  <dct:identifier>dct:title</dct:identifier>
		  <rdfs:domain rdf:resource="http://stelar-project.eu/klms#Category"/>
		  <rdfs:range rdf:resource="http://www.w3.org/2000/01/rdf-schema#Literal"/>
		  <rdfs:label xml:lang="en">Category - title</rdfs:label>
		  <rdfs:isDefinedBy rdf:resource="http://dublincore.org/documents/dcmi-terms/#terms-title" />
		  <rdfs:comment xml:lang="en">The name (title or type) of a class representing a category in a categorical distribution.</rdfs:comment>
	 </owl:DatatypeProperty>
-->
	 
	<owl:DatatypeProperty rdf:about="http://stelar-project.eu/klms#percentage"> 
		  <vann:usageNote xml:lang="en">Optional property. The percentage of instances of this class in a categorical distribution.</vann:usageNote>
		  <dct:identifier>klms:percentage</dct:identifier>
		  <rdfs:domain rdf:resource="http://stelar-project.eu/klms#Category"/>
		  <rdfs:range rdf:resource="http://www.w3.org/2001/XMLSchema#float"/>
		  <rdfs:label xml:lang="en">Category - percentage</rdfs:label>
		  <rdfs:comment xml:lang="en">The percentage of instances of this class in a categorical distribution.</rdfs:comment>
	 </owl:DatatypeProperty> 

	 
<!-- ============================================= -->
<!-- ==    DISTRIBUTION (KLMS) - Properties     == -->
<!-- ============================================= -->  
 
<!--  Distribution - access URL   -->
	 <owl:DatatypeProperty rdf:about="http://www.w3.org/ns/dcat#accessURL"> 
		  <vann:usageNote xml:lang="en">Mandatory property.  This property contains a URL that gives access to a Distribution of the Dataset. The resource at the access URL may contain information about how to get the Dataset. </vann:usageNote>
		  <dct:identifier>dcat:accessURL</dct:identifier>
		  <rdfs:label xml:lang="en">Distribution - access URL</rdfs:label>
		  <rdfs:domain rdf:resource="http://www.w3.org/ns/dcat#Distribution"/>
		  <rdfs:range rdf:resource="http://www.w3.org/2000/01/rdf-schema#Resource"/>
		  <rdfs:isDefinedBy rdf:resource="https://www.w3.org/TR/vocab-dcat-2/#Property:distribution_access_url" />
		  <rdfs:comment xml:lang="en">This property contains a URL that gives access to a Distribution of the Dataset. The resource at the access URL may contain information about how to get the Dataset.</rdfs:comment>
	 </owl:DatatypeProperty>

<!--  Distribution - description   -->
	 <owl:DatatypeProperty rdf:about="http://purl.org/dc/terms/description"> 
		  <vann:usageNote xml:lang="en">Recommended property. This property contains a free-text account of the Distribution. This property can be repeated for parallel language versions of the description.</vann:usageNote>
		  <dct:identifier>dct:description</dct:identifier>
		  <rdfs:domain rdf:resource="http://www.w3.org/ns/dcat#Distribution"/>
		  <rdfs:range rdf:resource="http://www.w3.org/2000/01/rdf-schema#Literal"/>
		  <rdfs:label xml:lang="en">Distribution - description</rdfs:label>
		  <rdfs:isDefinedBy rdf:resource="http://dublincore.org/documents/dcmi-terms/#terms-description" />
		  <rdfs:comment xml:lang="en">This property can be repeated for parallel language versions of the description.</rdfs:comment>
	 </owl:DatatypeProperty>
 
<!--  Distribution - format   -->
	 <owl:DatatypeProperty rdf:about="http://purl.org/dc/terms/format"> 
		  <vann:usageNote xml:lang="en">Recommended property. This property refers to the file format of the Distribution.</vann:usageNote>
		  <dct:identifier>dct:format</dct:identifier>
		  <rdfs:domain rdf:resource="http://www.w3.org/ns/dcat#Distribution"/>
		  <rdfs:range rdf:resource="http://purl.org/dc/terms/MediaTypeOrExtent"/>
		  <rdfs:label xml:lang="en">Distribution - format</rdfs:label>
		  <rdfs:isDefinedBy rdf:resource="http://dublincore.org/documents/dcmi-terms/#terms-format" />
		  <rdfs:comment xml:lang="en">This property refers to the file format of the Distribution.</rdfs:comment>
	 </owl:DatatypeProperty>
 
<!--  Distribution - license - N/A: Defined at the Dataset level in CKAN.  -->
<!--
	 <owl:DatatypeProperty rdf:about="http://purl.org/dc/terms/license"> 
	  <vann:usageNote xml:lang="en">Recommended property. This property refers to the license under which the Distribution is made available.</vann:usageNote>
	  <dct:identifier>dct:license</dct:identifier>
	  <rdfs:domain rdf:resource="http://www.w3.org/ns/dcat#Distribution"/>
	  <rdfs:range rdf:resource="http://purl.org/dc/terms/LicenseDocument"/>
	  <rdfs:label xml:lang="en">Distribution - license</rdfs:label>
	  <rdfs:isDefinedBy rdf:resource="http://dublincore.org/documents/dcmi-terms/#terms-license" />
	  <rdfs:comment xml:lang="en">This property refers to the license under which the Distribution is made available.</rdfs:comment>
	 </owl:DatatypeProperty>
-->
 
<!--  Distribution - byte size   -->
	 <owl:DatatypeProperty rdf:about="http://www.w3.org/ns/dcat#byteSize"> 
		  <vann:usageNote xml:lang="en">Optional property. This property contains the size of a Distribution in bytes.</vann:usageNote>
		  <dct:identifier>dcat:byteSize</dct:identifier>
		  <rdfs:domain rdf:resource="http://www.w3.org/ns/dcat#Distribution"/>
		  <rdfs:range rdf:resource="http://www.w3.org/2001/XMLSchema#decimal"/>
		  <rdfs:label xml:lang="en">Distribution - byte size</rdfs:label>
		  <rdfs:isDefinedBy rdf:resource="https://www.w3.org/TR/vocab-dcat-2/#Property:distribution_size" />
		  <rdfs:comment xml:lang="en">This property contains the size of a Distribution in bytes.</rdfs:comment>
	 </owl:DatatypeProperty>
 
<!--  Distribution - download URL   -->
	 <owl:ObjectProperty rdf:about="http://www.w3.org/ns/dcat#downloadURL"> 
		  <vann:usageNote xml:lang="en">Optional property. This property contains a URL that is direct link to a downloadable file in a given format.</vann:usageNote>
		  <dct:identifier>dcat:downloadURL</dct:identifier>
		  <rdfs:domain rdf:resource="http://www.w3.org/ns/dcat#Distribution"/>
		  <rdfs:range rdf:resource="http://www.w3.org/2000/01/rdf-schema#Resource"/>
		  <rdfs:label xml:lang="en">Distribution - download URL</rdfs:label>
		  <rdfs:isDefinedBy rdf:resource="https://www.w3.org/TR/vocab-dcat-2/#Property:distribution_download_url" />
		  <rdfs:comment xml:lang="en">This property contains a URL that is direct link to a downloadable file in a given format.</rdfs:comment>
	 </owl:ObjectProperty>
 
<!--  Distribution - media type   -->
	 <owl:ObjectProperty rdf:about="http://purl.org/dc/terms/mediaType"> 
		  <vann:usageNote xml:lang="en">Optional property. Subproperty of dct:format. This property refers to the media type of the Distribution if this is defined in IANA.</vann:usageNote>
		  <dct:identifier>dcat:mediaType</dct:identifier>
		  <rdfs:domain rdf:resource="http://www.w3.org/ns/dcat#Distribution"/>
		  <rdfs:range rdf:resource="http://purl.org/dc/terms/MediaType"/>
		  <rdfs:label xml:lang="en">Distribution - media type</rdfs:label>
		  <rdfs:isDefinedBy rdf:resource="http://dublincore.org/documents/dcmi-terms/#terms-mediaType" />
		  <rdfs:comment xml:lang="en">This property refers to the media type of the Distribution if this is defined in IANA.</rdfs:comment>
	 </owl:ObjectProperty>
 
<!--  Distribution - rights   -->
	 <owl:ObjectProperty rdf:about="http://purl.org/dc/terms/rights"> 
		  <vann:usageNote xml:lang="en">Optional property. This property refers to a statement that specifies rights associated with the Distribution.</vann:usageNote>
		  <dct:identifier>dct:rights</dct:identifier>
		  <rdfs:domain rdf:resource="http://www.w3.org/ns/dcat#Distribution"/>
		  <rdfs:range rdf:resource="http://purl.org/dc/terms/RightsStatement"/>
		  <rdfs:label xml:lang="en">Distribution - rights</rdfs:label>
		  <rdfs:isDefinedBy rdf:resource="http://dublincore.org/documents/dcmi-terms/#terms-rights" />
		  <rdfs:comment xml:lang="en">This property refers to a statement that specifies rights associated with the Distribution.</rdfs:comment>
	 </owl:ObjectProperty>
 
<!--  Distribution - title   -->
	 <owl:DatatypeProperty rdf:about="http://purl.org/dc/terms/title"> 
		  <vann:usageNote xml:lang="en">Optional property. This property contains a name given to the Distribution. This property can be repeated for parallel language versions of the description.</vann:usageNote>
		  <dct:identifier>dct:title</dct:identifier>
		  <rdfs:domain rdf:resource="http://www.w3.org/ns/dcat#Distribution"/>
		  <rdfs:range rdf:resource="http://www.w3.org/2000/01/rdf-schema#Literal"/>
		  <rdfs:label xml:lang="en">Distribution - title</rdfs:label>
		  <rdfs:isDefinedBy rdf:resource="http://dublincore.org/documents/dcmi-terms/#terms-title" />
		  <rdfs:comment xml:lang="en">This property contains a name given to the Distribution. This property can be repeated for parallel language versions of the description.</rdfs:comment>
	 </owl:DatatypeProperty>
 
 <!--  Distribution - keyword/ tag  -->
	 <owl:DatatypeProperty rdf:about="http://www.w3.org/ns/dcat#keyword"> 
		  <vann:usageNote xml:lang="en">Optional property. This property contains a keyword or tag describing the Distribution.</vann:usageNote>
		  <dct:identifier>dcat:keyword</dct:identifier>
		  <rdfs:domain rdf:resource="http://www.w3.org/ns/dcat#Distribution"/>
		  <rdfs:range rdf:resource="http://www.w3.org/2000/01/rdf-schema#Literal"/>
		  <rdfs:label xml:lang="en">Distribution - keyword/ tag</rdfs:label>
		  <rdfs:isDefinedBy rdf:resource="https://www.w3.org/TR/vocab-dcat-2/#Property:resource_keyword" />
		  <rdfs:comment xml:lang="en">This property contains a keyword or tag describing the Distribution.</rdfs:comment>
	 </owl:DatatypeProperty>
 
 <!--  Distribution - language   -->
	 <owl:ObjectProperty rdf:about="http://purl.org/dc/terms/language"> 
		  <vann:usageNote xml:lang="en">Optional property. This property refers to a language used in the Distribution. This property can be repeated if the metadata is provided in multiple languages.</vann:usageNote>
		  <dct:identifier>dct:language</dct:identifier>
		  <rdfs:label xml:lang="en">Distribution - language</rdfs:label>
		  <rdfs:domain rdf:resource="http://www.w3.org/ns/dcat#Distribution"/>
		  <rdfs:range rdf:resource="http://purl.org/dc/terms/LinguisticSystem"/>
		  <rdfs:isDefinedBy rdf:resource="http://dublincore.org/documents/dcmi-terms/#terms-language" />
		  <rdfs:comment xml:lang="en">This property refers to a language used in the Distribution.</rdfs:comment> 
	 </owl:ObjectProperty>  
	 
 <!--  Distribution - linked schemas   -->
	 <owl:ObjectProperty rdf:about="http://purl.org/dc/terms/conformsTo"> 
		  <vann:usageNote xml:lang="en">Optional property. This property refers to an established schema to which the described Distribution conforms.</vann:usageNote>
		  <dct:identifier>dct:conformsTo</dct:identifier>
		  <rdfs:domain rdf:resource="http://www.w3.org/ns/dcat#Distribution"/>
		  <rdfs:label xml:lang="en">Distribution - linked schemas</rdfs:label>
		  <rdfs:range rdf:resource="http://purl.org/dc/terms/Standard"/>
		  <rdfs:isDefinedBy rdf:resource="http://dublincore.org/documents/dcmi-terms/#terms-conformsTo" />
		  <rdfs:comment xml:lang="en">This property refers to an established schema to which the described Distribution conforms.</rdfs:comment> 
	 </owl:ObjectProperty>	 
	 
 <!--  Distribution - release date   -->
	 <owl:DatatypeProperty rdf:about="http://purl.org/dc/terms/issued"> 
		  <vann:usageNote xml:lang="en">Optional property. This property contains the date of formal issuance (e.g., publication) of the Distribution.</vann:usageNote>
		  <dct:identifier>dct:issued</dct:identifier>
		  <rdfs:domain rdf:resource="http://www.w3.org/ns/dcat#Distribution"/>
		  <rdfs:range rdf:resource="http://www.w3.org/2001/XMLSchema#dateTime"/>
		  <rdfs:label xml:lang="en">Distribution - release date</rdfs:label>
		  <rdfs:isDefinedBy rdf:resource="http://dublincore.org/documents/dcmi-terms/#terms-issued" />
		  <rdfs:comment xml:lang="en">This property contains the date of formal issuance (e.g., publication) of the Distribution.</rdfs:comment>
	 </owl:DatatypeProperty>
	 
<!--  Distribution - update/modification date   -->
	 <owl:DatatypeProperty rdf:about="http://purl.org/dc/terms/modified"> 
		  <vann:usageNote xml:lang="en">Optional property. This property contains the most recent date on which the Distribution was changed or modified.</vann:usageNote>
		  <dct:identifier>dct:modified</dct:identifier>
		  <rdfs:domain rdf:resource="http://www.w3.org/ns/dcat#Distribution"/>
		  <rdfs:range rdf:resource="http://www.w3.org/2001/XMLSchema#dateTime"/>
		  <rdfs:label xml:lang="en">Distribution - update/modification date</rdfs:label>
		  <rdfs:isDefinedBy rdf:resource="http://dublincore.org/documents/dcmi-terms/#terms-modified" />
		  <rdfs:comment xml:lang="en">This property contains the most recent date on which the Distribution was changed or modified.</rdfs:comment>
	 </owl:DatatypeProperty>

 <!--  Distribution - documentation   -->
	 <owl:ObjectProperty rdf:about="http://xmlns.com/foaf/0.1/page"> 
		  <vann:usageNote xml:lang="en">Optional property.This property refers to a page or document about this Distribution.</vann:usageNote>
		  <dct:identifier>foaf:page</dct:identifier>
		  <rdfs:domain rdf:resource="http://www.w3.org/ns/dcat#Distribution"/>
		  <rdfs:range rdf:resource="http://xmlns.com/foaf/0.1/Document"/>
		  <rdfs:label xml:lang="en">Distribution - documentation</rdfs:label>
		  <rdfs:isDefinedBy rdf:resource="http://xmlns.com/foaf/spec/#term_page" />
		  <rdfs:comment xml:lang="en">This property refers to a page or document about this Distribution.</rdfs:comment>
	 </owl:ObjectProperty>


<!--  Distribution - profile URL   -->
    <owl:DatatypeProperty rdf:about="http://stelar-project.eu/klms#profileURL"> 
        <rdfs:label xml:lang="en">Distribution - Profile URL</rdfs:label>
        <dct:identifier>klms:profileURL</dct:identifier>
        <rdfs:domain rdf:resource="http://stelar-project.eu/klms#Distribution"/>
        <rdfs:range rdf:resource="http://www.w3.org/2000/01/rdf-schema#Resource"/>
        <vann:usageNote xml:lang="en">Optional property. This property can be used to store a link to a file or web application that contains all the profiling results.</vann:usageNote>
        <rdfs:comment xml:lang="en">This property can be used to store a link to a file or web application that contains all the profiling results.</rdfs:comment>
    </owl:DatatypeProperty>


<!-- ====================================== -->
<!-- ==        RASTER - Properties       == -->
<!-- ====================================== -->  

<!-- http://stelar-project.eu/klms#height -->
    <owl:DatatypeProperty rdf:about="http://stelar-project.eu/klms#height">
        <rdfs:domain rdf:resource="http://stelar-project.eu/klms#Raster"/>
        <rdfs:range rdf:resource="http://www.w3.org/2001/XMLSchema#int"/>
        <dct:identifier>klms:height</dct:identifier>
        <rdfs:label xml:lang="en">Raster - Raster Image Height</rdfs:label>
        <vann:usageNote xml:lang="en">Optional property. This property describes the height of a raster image in pixels.</vann:usageNote>
        <rdfs:comment xml:lang="en">The height of a raster image in pixels.</rdfs:comment>
    </owl:DatatypeProperty>
    
<!-- http://stelar-project.eu/klms#width -->
    <owl:DatatypeProperty rdf:about="http://stelar-project.eu/klms#width">
        <rdfs:domain rdf:resource="http://stelar-project.eu/klms#Raster"/>
        <rdfs:range rdf:resource="http://www.w3.org/2001/XMLSchema#int"/>
        <dct:identifier>klms:width</dct:identifier>
        <rdfs:label xml:lang="en">Raster - Raster Image Width</rdfs:label>
        <vann:usageNote xml:lang="en">Optional property. This property describes the width of a raster image in pixels.</vann:usageNote>
        <rdfs:comment xml:lang="en">The width of a raster image in pixels.</rdfs:comment>
    </owl:DatatypeProperty>

<!-- http://stelar-project.eu/klms#crs -->
    <owl:DatatypeProperty rdf:about="http://stelar-project.eu/klms#crs">
        <rdfs:range rdf:resource="http://www.w3.org/2001/XMLSchema#string"/>
        <dct:identifier>klms:crs</dct:identifier>
        <rdfs:label xml:lang="en">Geospatial - CRS</rdfs:label>
        <vann:usageNote xml:lang="en">Optional property. This property describes the CRS of a geospatial dataset.</vann:usageNote>
        <rdfs:comment xml:lang="en">The CRS of a geospatial dataset.</rdfs:comment>
    </owl:DatatypeProperty>

<!-- http://stelar-project.eu/klms#noDataValue -->
     <owl:DatatypeProperty rdf:about="http://www.w3.org/ns/dcat#noDataValue">
        <rdfs:domain rdf:resource="http://stelar-project.eu/klms#Raster"/>
        <rdfs:range rdf:resource="http://www.w3.org/2001/XMLSchema#string"/>
        <dct:identifier>klms:noDataValue</dct:identifier>
        <rdfs:label xml:lang="en">Raster - No data value</rdfs:label>
        <vann:usageNote xml:lang="en">Optional property. This property describes the no-data value for a raster image.</vann:usageNote>
        <rdfs:comment xml:lang="en">The no-data value for a raster image.</rdfs:comment>
     </owl:DatatypeProperty>
 
 <!--  Raster - temporal resolution -->
	 <owl:DatatypeProperty rdf:about="http://www.w3.org/ns/dcat#temporalResolution"> 
	  <vann:usageNote xml:lang="en">Optional property. This property refers to the minimum time period resolvable in a raster dataset. </vann:usageNote>
	  <dct:identifier>dcat:temporalResolution</dct:identifier>
	  <rdfs:label xml:lang="en">Raster - temporal resolution </rdfs:label>
	  <rdfs:domain rdf:resource="http://stelar-project.eu/klms#Raster"/>
	  <rdfs:range rdf:resource="http://www.w3.org/2001/XMLSchema#duration"/>
	  <rdfs:isDefinedBy rdf:resource="https://www.w3.org/TR/vocab-dcat-2/#Property:dataset_temporal_resolution" />
	  <rdfs:comment xml:lang="en">This property refers to the minimum time period resolvable in a raster dataset. If the dataset is a time-series this should correspond to the spacing of items in the series. For other kinds of dataset, this property will usually indicate the smallest time difference between items in the dataset.</rdfs:comment>
	 </owl:DatatypeProperty>
  
 <!--  Raster - spatial resolution -->
	 <owl:DatatypeProperty rdf:about="http://www.w3.org/ns/dcat#spatialResolutionInMeters"> 
	  <vann:usageNote xml:lang="en">Optional property. This property refers to the minimum spatial separation resolvable in a raster dataset, measured in meters. </vann:usageNote>
	  <dct:identifier>dcat:spatialResolutionInMeters</dct:identifier>
	  <rdfs:label xml:lang="en">Raster - spatial resolution</rdfs:label>
	  <rdfs:domain rdf:resource="http://stelar-project.eu/klms#Raster"/>
	  <rdfs:range rdf:resource="http://www.w3.org/2001/XMLSchema#decimal"/>
	  <rdfs:isDefinedBy rdf:resource="https://www.w3.org/TR/vocab-dcat-2/#Property:dataset_spatial_resolution" />
	  <rdfs:comment xml:lang="en">This property refers to the  minimum spatial separation resolvable in a raster dataset, measured in meters.</rdfs:comment>
	 </owl:DatatypeProperty>


<!-- ====================================== -->
<!-- ==       TABULAR - Properties       == -->
<!-- ====================================== -->  

<!-- http://stelar-project.eu/klms#numColumns -->
    <owl:DatatypeProperty rdf:about="http://stelar-project.eu/klms#numColumns">
        <rdfs:domain rdf:resource="http://stelar-project.eu/klms#Tabular"/>
        <rdfs:range rdf:resource="http://www.w3.org/2001/XMLSchema#int"/>
        <dct:identifier>klms:numColumns</dct:identifier>
        <rdfs:label xml:lang="en">Tabular - Number of Columns</rdfs:label>
        <vann:usageNote xml:lang="en">Optional property. This property describes the number of columns of a tabular dataset.</vann:usageNote>
        <rdfs:comment xml:lang="en">The number of columns of a tabular dataset.</rdfs:comment>
    </owl:DatatypeProperty>
    
<!-- http://stelar-project.eu/klms#numRows -->
    <owl:DatatypeProperty rdf:about="http://stelar-project.eu/klms#numRows">
        <rdfs:domain rdf:resource="http://stelar-project.eu/klms#Tabular"/>
        <rdfs:range rdf:resource="http://www.w3.org/2001/XMLSchema#int"/>
        <dct:identifier>klms:numRows</dct:identifier>
        <rdfs:label xml:lang="en">Tabular - Number of Rows</rdfs:label>
        <vann:usageNote xml:lang="en">Optional property. This property describes the number of rows of a tabular dataset.</vann:usageNote>
        <rdfs:comment xml:lang="en">The number of rows of a tabular dataset.</rdfs:comment>
    </owl:DatatypeProperty>



<!-- ====================================== -->
<!-- ==    HIERARCHICAL - Properties     == -->
<!-- ====================================== --> 

<!-- http://stelar-project.eu/klms#numRecords -->
    <owl:DatatypeProperty rdf:about="http://stelar-project.eu/klms#numRecords">
        <rdfs:domain rdf:resource="http://stelar-project.eu/klms#Hierarchical"/>
        <rdfs:range rdf:resource="http://www.w3.org/2001/XMLSchema#int"/>
        <dct:identifier>klms:numRecords</dct:identifier>
        <rdfs:label xml:lang="en">Hierarchical - Number of records</rdfs:label>
        <vann:usageNote xml:lang="en">Optional property. This property describes the number of records of a hierarchical dataset.</vann:usageNote>
        <rdfs:comment xml:lang="en">The number of records of a hierarchical dataset.</rdfs:comment>
    </owl:DatatypeProperty>
    
<!-- http://stelar-project.eu/klms#numAttributes -->
    <owl:DatatypeProperty rdf:about="http://stelar-project.eu/klms#numAttributes">
        <rdfs:domain rdf:resource="http://stelar-project.eu/klms#Hierarchical"/>
        <rdfs:range rdf:resource="http://www.w3.org/2001/XMLSchema#int"/>
        <dct:identifier>klms:numAttributes</dct:identifier>
        <rdfs:label xml:lang="en">Tabular - Number of attributes</rdfs:label>
        <vann:usageNote xml:lang="en">Optional property. This property describes the number of attributes of a hierarchical dataset.</vann:usageNote>
        <rdfs:comment xml:lang="en">The number of attributes of a hierarchical dataset.</rdfs:comment>
    </owl:DatatypeProperty>


<!-- ====================================== -->
<!-- ==      RDFGraph - Properties       == -->
<!-- ====================================== --> 

<!-- http://stelar-project.eu/klms#numNamespaces -->
    <owl:DatatypeProperty rdf:about="http://stelar-project.eu/klms#numNamespaces">
        <rdfs:domain rdf:resource="http://stelar-project.eu/klms#RDFGraph"/>
        <rdfs:range rdf:resource="http://www.w3.org/2001/XMLSchema#int"/>
        <dct:identifier>klms:numNamespaces</dct:identifier>
        <rdfs:label xml:lang="en">RDFGraph - Number of namespaces</rdfs:label>
        <vann:usageNote xml:lang="en">Optional property. This property describes the number of namespaces of an RDF graph dataset.</vann:usageNote>
        <rdfs:comment xml:lang="en">The number of namespaces of an RDF graph dataset.</rdfs:comment>
    </owl:DatatypeProperty>
    
<!-- http://stelar-project.eu/klms#numClasses -->
    <owl:DatatypeProperty rdf:about="http://stelar-project.eu/klms#numClasses">
        <rdfs:domain rdf:resource="http://stelar-project.eu/klms#RDFGraph"/>
        <rdfs:range rdf:resource="http://www.w3.org/2001/XMLSchema#int"/>
        <dct:identifier>klms:numClasses</dct:identifier>
        <rdfs:label xml:lang="en">RDFGraph - Number of classes</rdfs:label>
        <vann:usageNote xml:lang="en">Optional property. This property describes the number of classes of an RDF graph dataset.</vann:usageNote>
        <rdfs:comment xml:lang="en">The number of classes of an RDF graph dataset.</rdfs:comment>
    </owl:DatatypeProperty>

<!-- http://stelar-project.eu/klms#numObjectProperties -->
    <owl:DatatypeProperty rdf:about="http://stelar-project.eu/klms#numObjectProperties">
        <rdfs:domain rdf:resource="http://stelar-project.eu/klms#RDFGraph"/>
        <rdfs:range rdf:resource="http://www.w3.org/2001/XMLSchema#int"/>
        <dct:identifier>klms:numObjectProperties</dct:identifier>
        <rdfs:label xml:lang="en">RDFGraph - Number of object properties</rdfs:label>
        <vann:usageNote xml:lang="en">Optional property. This property describes the number of object properties of an RDF graph dataset.</vann:usageNote>
        <rdfs:comment xml:lang="en">The number of object properties of an RDF graph dataset.</rdfs:comment>
    </owl:DatatypeProperty>

<!-- http://stelar-project.eu/klms#numDatatypeProperties -->
    <owl:DatatypeProperty rdf:about="http://stelar-project.eu/klms#numDatatypeProperties">
        <rdfs:domain rdf:resource="http://stelar-project.eu/klms#RDFGraph"/>
        <rdfs:range rdf:resource="http://www.w3.org/2001/XMLSchema#int"/>
        <dct:identifier>klms:numDatatypeProperties</dct:identifier>
        <rdfs:label xml:lang="en">RDFGraph - Number of datatype properties</rdfs:label>
        <vann:usageNote xml:lang="en">Optional property. This property describes the number of datatype properties of an RDF graph dataset.</vann:usageNote>
        <rdfs:comment xml:lang="en">The number of datatype properties of an RDF graph dataset.</rdfs:comment>
    </owl:DatatypeProperty>


<!-- ================================================ -->
<!-- ==   TEXT / TEXTUAL ATTRIBUTE - Properties    == -->
<!-- ================================================ -->

<!-- http://stelar-project.eu/klms#language -->
    <owl:DatatypeProperty rdf:about="http://stelar-project.eu/klms#language">
        <rdfs:domain rdf:resource="http://stelar-project.eu/klms#Text"/>
        <rdfs:range rdf:resource="http://www.w3.org/2001/XMLSchema#int"/>
        <dct:identifier>klms:language</dct:identifier>
        <rdfs:label xml:lang="en">Text - Main language</rdfs:label>
        <vann:usageNote xml:lang="en">Optional property. This property describes the language of a textual dataset.</vann:usageNote>
        <rdfs:comment xml:lang="en">The language of a textual dataset.</rdfs:comment>
    </owl:DatatypeProperty>

<!-- http://stelar-project.eu/klms#numSentences -->
    <owl:DatatypeProperty rdf:about="http://stelar-project.eu/klms#numSentences">
        <rdfs:domain rdf:resource="http://stelar-project.eu/klms#Text"/>
        <rdfs:range rdf:resource="http://www.w3.org/2001/XMLSchema#int"/>
        <dct:identifier>klms:numSentences</dct:identifier>
        <rdfs:label xml:lang="en">Text - Number of Sentences</rdfs:label>
        <vann:usageNote xml:lang="en">Optional property. This property describes the number of sentences in a textual dataset.</vann:usageNote>
        <rdfs:comment xml:lang="en">The number of sentences in a textual dataset.</rdfs:comment>
    </owl:DatatypeProperty>

<!-- http://stelar-project.eu/klms#numWords -->
    <owl:DatatypeProperty rdf:about="http://stelar-project.eu/klms#numWords">
        <rdfs:domain rdf:resource="http://stelar-project.eu/klms#Text"/>
        <rdfs:range rdf:resource="http://www.w3.org/2001/XMLSchema#int"/>
        <dct:identifier>klms:numWords</dct:identifier>
        <rdfs:label xml:lang="en">Text - Number of words</rdfs:label>
        <vann:usageNote xml:lang="en">Optional property. This property describes the number of words in a textual dataset.</vann:usageNote>
        <rdfs:comment xml:lang="en">The number of words in a textual dataset.</rdfs:comment>
    </owl:DatatypeProperty>

<!-- http://stelar-project.eu/klms#numDistinctWords -->
    <owl:DatatypeProperty rdf:about="http://stelar-project.eu/klms#numDistinctWords">
        <rdfs:domain rdf:resource="http://stelar-project.eu/klms#Text"/>
        <rdfs:range rdf:resource="http://www.w3.org/2001/XMLSchema#int"/>
        <dct:identifier>klms:numDistinctWords</dct:identifier>
        <rdfs:label xml:lang="en">Text - Number of distinct words</rdfs:label>
        <vann:usageNote xml:lang="en">Optional property. This property describes the number of distinct words in a textual dataset.</vann:usageNote>
        <rdfs:comment xml:lang="en">The number of distinct words in a textual dataset.</rdfs:comment>
    </owl:DatatypeProperty>

<!-- http://stelar-project.eu/klms#numCharacters -->
    <owl:DatatypeProperty rdf:about="http://stelar-project.eu/klms#numCharacters">
        <rdfs:domain rdf:resource="http://stelar-project.eu/klms#Text"/>
        <rdfs:range rdf:resource="http://www.w3.org/2001/XMLSchema#int"/>
        <dct:identifier>klms:numCharacters</dct:identifier>
        <rdfs:label xml:lang="en">Text - Number of characters</rdfs:label>
        <vann:usageNote xml:lang="en">Optional property. This property describes the number of characters in a textual dataset.</vann:usageNote>
        <rdfs:comment xml:lang="en">The number of characters in a textual dataset.</rdfs:comment>
    </owl:DatatypeProperty>

<!-- http://stelar-project.eu/klms#ratioUppercase -->
    <owl:DatatypeProperty rdf:about="http://stelar-project.eu/klms#ratioUppercase">
        <rdfs:domain rdf:resource="http://stelar-project.eu/klms#Text"/>
        <rdfs:domain rdf:resource="http://stelar-project.eu/klms#TextualAttribute"/>
        <rdfs:range rdf:resource="http://www.w3.org/2001/XMLSchema#float"/>
        <dct:identifier>klms:ratioUppercase</dct:identifier>
        <rdfs:label xml:lang="en">Text - Ratio uppercase</rdfs:label>
        <vann:usageNote xml:lang="en">Optional property. This property describes the ratio of uppercase letters in a textual dataset.</vann:usageNote>
        <rdfs:comment xml:lang="en">The ratio of uppercase letters in a textual dataset.</rdfs:comment>
    </owl:DatatypeProperty>

<!-- http://stelar-project.eu/klms#ratioDigits -->
    <owl:DatatypeProperty rdf:about="http://stelar-project.eu/klms#ratioDigits">
        <rdfs:domain rdf:resource="http://stelar-project.eu/klms#Text"/>
        <rdfs:domain rdf:resource="http://stelar-project.eu/klms#TextualAttribute"/>
        <rdfs:range rdf:resource="http://www.w3.org/2001/XMLSchema#float"/>
        <dct:identifier>klms:ratioDigits</dct:identifier>
        <rdfs:label xml:lang="en">Text - Ratio digits</rdfs:label>
        <vann:usageNote xml:lang="en">Optional property. This property describes the ratio of digits in a textual dataset.</vann:usageNote>
        <rdfs:comment xml:lang="en">The ratio of digits in a textual dataset.</rdfs:comment>
    </owl:DatatypeProperty>

<!-- http://stelar-project.eu/klms#ratioSpecialChars -->
    <owl:DatatypeProperty rdf:about="http://stelar-project.eu/klms#ratioSpecialChars">
        <rdfs:domain rdf:resource="http://stelar-project.eu/klms#Text"/>
        <rdfs:domain rdf:resource="http://stelar-project.eu/klms#TextualAttribute"/>
        <rdfs:range rdf:resource="http://www.w3.org/2001/XMLSchema#float"/>
        <dct:identifier>klms:ratioSpecialChars</dct:identifier>
        <rdfs:label xml:lang="en">Text - Ratio special characters</rdfs:label>
        <vann:usageNote xml:lang="en">Optional property. This property describes the ratio of special characters in a textual dataset.</vann:usageNote>
        <rdfs:comment xml:lang="en">The ratio of special characters in a textual dataset.</rdfs:comment>
    </owl:DatatypeProperty>


<!-- ====================================== -->
<!-- ==    ATTRIBUTE - Properties        == -->
<!-- ====================================== -->

<!-- http://stelar-project.eu/klms#type -->
    <owl:DatatypeProperty rdf:about="http://stelar-project.eu/klms#type">
        <rdfs:domain rdf:resource="http://stelar-project.eu/klms#Attribute"/>
        <rdfs:range rdf:resource="http://www.w3.org/2001/XMLSchema#string"/>
        <dct:identifier>klms:type</dct:identifier>
        <rdfs:label xml:lang="en">Attribute - Type</rdfs:label>
        <vann:usageNote xml:lang="en">Optional property. This property describes the type of an attribute.</vann:usageNote>
        <rdfs:comment xml:lang="en">The type of an attribute.</rdfs:comment>
    </owl:DatatypeProperty>

<!-- http://stelar-project.eu/klms#missingRatio -->
    <owl:DatatypeProperty rdf:about="http://stelar-project.eu/klms#missingRatio">
        <rdfs:domain rdf:resource="http://stelar-project.eu/klms#Attribute"/>
        <rdfs:range rdf:resource="http://www.w3.org/2001/XMLSchema#float"/>
        <dct:identifier>klms:missingRatio</dct:identifier>
        <rdfs:label xml:lang="en">Attribute - Missing values ratio</rdfs:label>
        <vann:usageNote xml:lang="en">Optional property. This property describes the missing values ratio of an attribute.</vann:usageNote>
        <rdfs:comment xml:lang="en">The missing values ratio of an attribute.</rdfs:comment>
    </owl:DatatypeProperty>

<!-- http://stelar-project.eu/klms#uniqueness -->
    <owl:DatatypeProperty rdf:about="http://stelar-project.eu/klms#uniqueness">
        <rdfs:domain rdf:resource="http://stelar-project.eu/klms#Attribute"/>
        <rdfs:range rdf:resource="http://www.w3.org/2001/XMLSchema#float"/>
        <dct:identifier>klms:uniqueness</dct:identifier>
        <rdfs:label xml:lang="en">Attribute - Uniqueness</rdfs:label>
        <vann:usageNote xml:lang="en">Optional property. This property describes the number of distinct values divided by the number of total values of an attribute.</vann:usageNote>
        <rdfs:comment xml:lang="en">The number of distinct values divided by the number of total values of an attribute.</rdfs:comment>
    </owl:DatatypeProperty>

<!-- http://stelar-project.eu/klms#nestingLevel -->
    <owl:DatatypeProperty rdf:about="http://stelar-project.eu/klms#nestingLevel">
        <rdfs:domain rdf:resource="http://stelar-project.eu/klms#Attribute"/>
        <rdfs:range rdf:resource="http://www.w3.org/2001/XMLSchema#int"/>
        <dct:identifier>klms:nestingLevel</dct:identifier>
        <rdfs:label xml:lang="en">Attribute - Nesting Level</rdfs:label>
        <vann:usageNote xml:lang="en">Optional property. This property describes the nesting of the attribute (in case of nested attributes or property hierarchies).</vann:usageNote>
        <rdfs:comment xml:lang="en">The nesting of the attribute.</rdfs:comment>
    </owl:DatatypeProperty>



<!-- ================================================= -->
<!-- ==    SERIES ATTRIBUTE - Properties            == -->
<!-- ================================================= -->

<!-- http://stelar-project.eu/klms#absEnergy -->
    <owl:DatatypeProperty rdf:about="http://stelar-project.eu/klms#absEnergy">
        <rdfs:domain rdf:resource="http://stelar-project.eu/klms#SeriesAttribute"/>
        <rdfs:range rdf:resource="http://www.w3.org/2001/XMLSchema#float"/>
        <dct:identifier>klms:absEnergy</dct:identifier>
        <rdfs:label xml:lang="en">SeriesAttribute - Absolute energy</rdfs:label>
        <vann:usageNote xml:lang="en">Optional property. This property can be used describe the absolute energy of a series dataset.</vann:usageNote>
        <rdfs:comment xml:lang="en">The absolute energy of a series dataset.</rdfs:comment>
    </owl:DatatypeProperty>

<!-- http://stelar-project.eu/klms#absSumChanges -->
    <owl:DatatypeProperty rdf:about="http://stelar-project.eu/klms#absSumChanges">
        <rdfs:domain rdf:resource="http://stelar-project.eu/klms#SeriesAttribute"/>
        <rdfs:range rdf:resource="http://www.w3.org/2001/XMLSchema#float"/>
        <dct:identifier>klms:absSumChanges</dct:identifier>
        <rdfs:label xml:lang="en">SeriesAttribute - Absolute sum of changes</rdfs:label>
        <vann:usageNote xml:lang="en">Optional property. This property can be used describe the absolute value of consecutive changes of a series dataset.</vann:usageNote>
        <rdfs:comment xml:lang="en">The absolute value of consecutive changes of a series dataset.</rdfs:comment>
    </owl:DatatypeProperty>

<!-- http://stelar-project.eu/klms#lenAboveMean -->
    <owl:DatatypeProperty rdf:about="http://stelar-project.eu/klms#lenAboveMean">
        <rdfs:domain rdf:resource="http://stelar-project.eu/klms#SeriesAttribute"/>
        <rdfs:range rdf:resource="http://www.w3.org/2001/XMLSchema#int"/>
        <dct:identifier>klms:lenAboveMean</dct:identifier>
        <rdfs:label xml:lang="en">SeriesAttribute - Maximum subsequence length above mean</rdfs:label>
        <vann:usageNote xml:lang="en">Optional property. This property can be used describe the length of the longest subsequence above the mean value of a series dataset.</vann:usageNote>
        <rdfs:comment xml:lang="en">The longest subsequence above the mean value.</rdfs:comment>
    </owl:DatatypeProperty>

<!-- http://stelar-project.eu/klms#lenBelowMean -->
    <owl:DatatypeProperty rdf:about="http://stelar-project.eu/klms#lenBelowMean">
        <rdfs:domain rdf:resource="http://stelar-project.eu/klms#SeriesAttribute"/>
        <rdfs:range rdf:resource="http://www.w3.org/2001/XMLSchema#int"/>
        <dct:identifier>klms:lenBelowMean</dct:identifier>
        <rdfs:label xml:lang="en">SeriesAttribute - Maximum subsequence length below mean</rdfs:label>
        <vann:usageNote xml:lang="en">Optional property. This property can be used describe the length of the longest subsequence below the mean value of a series dataset.</vann:usageNote>
        <rdfs:comment xml:lang="en">The longest subsequence below the mean value.</rdfs:comment>
    </owl:DatatypeProperty>

<!-- http://stelar-project.eu/klms#numPeaks -->
    <owl:DatatypeProperty rdf:about="http://stelar-project.eu/klms#numPeaks">
        <rdfs:domain rdf:resource="http://stelar-project.eu/klms#SeriesAttribute"/>
        <rdfs:range rdf:resource="http://www.w3.org/2001/XMLSchema#int"/>
        <dct:identifier>klms:numPeaks</dct:identifier>
        <rdfs:label xml:lang="en">SeriesAttribute - Number of peaks</rdfs:label>
        <vann:usageNote xml:lang="en">Optional property. This property can be used describe the total number of peaks of a series dataset.</vann:usageNote>
        <rdfs:comment xml:lang="en">The total number of peaks of a series dataset.</rdfs:comment>
    </owl:DatatypeProperty>


<!-- ================================================= -->
<!-- ==    NUMERICAL DISTRIBUTION - Properties      == -->
<!-- ================================================= -->

<!-- http://stelar-project.eu/klms#min -->
    <owl:DatatypeProperty rdf:about="http://stelar-project.eu/klms#min">
        <rdfs:domain rdf:resource="http://stelar-project.eu/klms#NumericalDistribution"/>
        <rdfs:range rdf:resource="http://www.w3.org/2001/XMLSchema#float"/>
        <dct:identifier>klms:min</dct:identifier>
        <rdfs:label xml:lang="en">NumericalDistribution - Minimum value</rdfs:label>
        <vann:usageNote xml:lang="en">Optional property. This property can be used describe a minimum value.</vann:usageNote>
        <rdfs:comment xml:lang="en">A minimum value.</rdfs:comment>
    </owl:DatatypeProperty>

<!-- http://stelar-project.eu/klms#max -->
    <owl:DatatypeProperty rdf:about="http://stelar-project.eu/klms#max">
        <rdfs:domain rdf:resource="http://stelar-project.eu/klms#NumericalDistribution"/>
        <rdfs:range rdf:resource="http://www.w3.org/2001/XMLSchema#float"/>
        <dct:identifier>klms:max</dct:identifier>
        <rdfs:label xml:lang="en">NumericalDistribution - Maximum value</rdfs:label>
        <vann:usageNote xml:lang="en">Optional property. This property can be used describe a maximum value.</vann:usageNote>
        <rdfs:comment xml:lang="en">A maximum value.</rdfs:comment>
    </owl:DatatypeProperty>

<!-- http://stelar-project.eu/klms#count -->
    <owl:DatatypeProperty rdf:about="http://stelar-project.eu/klms#count">
        <rdfs:range rdf:resource="http://www.w3.org/2001/XMLSchema#int"/>
        <dct:identifier>klms:count</dct:identifier>
        <rdfs:label xml:lang="en">NumericalDistribution/Category - Count</rdfs:label>
        <vann:usageNote xml:lang="en">Optional property. This property can be used describe a count.</vann:usageNote>
        <rdfs:comment xml:lang="en">A count.</rdfs:comment>
    </owl:DatatypeProperty>

<!-- http://stelar-project.eu/klms#average -->
    <owl:DatatypeProperty rdf:about="http://stelar-project.eu/klms#average">
        <rdfs:domain rdf:resource="http://stelar-project.eu/klms#NumericalDistribution"/>
        <rdfs:range rdf:resource="http://www.w3.org/2001/XMLSchema#float"/>
        <dct:identifier>klms:average</dct:identifier>
        <rdfs:label xml:lang="en">NumericalDistribution - Average value</rdfs:label>
        <vann:usageNote xml:lang="en">Optional property. This property can be used describe an average value.</vann:usageNote>
        <rdfs:comment xml:lang="en">An average value.</rdfs:comment>
    </owl:DatatypeProperty>

<!-- http://stelar-project.eu/klms#stddev -->
    <owl:DatatypeProperty rdf:about="http://stelar-project.eu/klms#stddev">
        <rdfs:domain rdf:resource="http://stelar-project.eu/klms#NumericalDistribution"/>
        <rdfs:range rdf:resource="http://www.w3.org/2001/XMLSchema#float"/>
        <dct:identifier>klms:stddev</dct:identifier>
        <rdfs:label xml:lang="en">NumericalDistribution - Standard deviation</rdfs:label>
        <vann:usageNote xml:lang="en">Optional property. This property can be used describe a standard deviation value.</vann:usageNote>
        <rdfs:comment xml:lang="en">A standard deviation value.</rdfs:comment>
    </owl:DatatypeProperty>

<!-- http://stelar-project.eu/klms#median -->
    <owl:DatatypeProperty rdf:about="http://stelar-project.eu/klms#median">
        <rdfs:domain rdf:resource="http://stelar-project.eu/klms#NumericalDistribution"/>
        <rdfs:range rdf:resource="http://www.w3.org/2001/XMLSchema#float"/>
        <dct:identifier>klms:median</dct:identifier>
        <rdfs:label xml:lang="en">NumericalDistribution - Median</rdfs:label>
        <vann:usageNote xml:lang="en">Optional property. This property can be used describe a median value.</vann:usageNote>
        <rdfs:comment xml:lang="en">A median value.</rdfs:comment>
    </owl:DatatypeProperty>

<!-- http://stelar-project.eu/klms#kurtosis -->
    <owl:DatatypeProperty rdf:about="http://stelar-project.eu/klms#kurtosis">
        <rdfs:domain rdf:resource="http://stelar-project.eu/klms#NumericalDistribution"/>
        <rdfs:range rdf:resource="http://www.w3.org/2001/XMLSchema#float"/>
        <dct:identifier>klms:kurtosis</dct:identifier>
        <rdfs:label xml:lang="en">NumericalDistribution - Kurtosis</rdfs:label>
        <vann:usageNote xml:lang="en">Optional property. This property can be used describe the kurtosis of a collection of numbers.</vann:usageNote>
        <rdfs:comment xml:lang="en">The kurtosis of a collection of numbers.</rdfs:comment>
    </owl:DatatypeProperty>
    
<!-- http://stelar-project.eu/klms#skewness -->
    <owl:DatatypeProperty rdf:about="http://stelar-project.eu/klms#skewness">
        <rdfs:domain rdf:resource="http://stelar-project.eu/klms#NumericalDistribution"/>
        <rdfs:range rdf:resource="http://www.w3.org/2001/XMLSchema#float"/>
        <dct:identifier>klms:skewness</dct:identifier>
        <rdfs:label xml:lang="en">NumericalDistribution - Skewness</rdfs:label>
        <vann:usageNote xml:lang="en">Optional property. This property can be used describe the skewness of a collection of numbers.</vann:usageNote>
        <rdfs:comment xml:lang="en">The skewness of a collection of numbers.</rdfs:comment>
    </owl:DatatypeProperty>

<!-- http://stelar-project.eu/klms#variance -->
    <owl:DatatypeProperty rdf:about="http://stelar-project.eu/klms#variance">
        <rdfs:domain rdf:resource="http://stelar-project.eu/klms#NumericalDistribution"/>
        <rdfs:range rdf:resource="http://www.w3.org/2001/XMLSchema#float"/>
        <dct:identifier>klms:variance</dct:identifier>
        <rdfs:label xml:lang="en">NumericalDistribution - Variance</rdfs:label>
        <vann:usageNote xml:lang="en">Optional property. This property can be used describe the variance of a collection of numbers.</vann:usageNote>
        <rdfs:comment xml:lang="en">The variance of a collection of numbers.</rdfs:comment>
    </owl:DatatypeProperty>

<!-- http://stelar-project.eu/klms#percentile10 -->
    <owl:DatatypeProperty rdf:about="http://stelar-project.eu/klms#percentile10">
        <rdfs:domain rdf:resource="http://stelar-project.eu/klms#NumericalDistribution"/>
        <rdfs:range rdf:resource="http://www.w3.org/2001/XMLSchema#float"/>
        <dct:identifier>klms:percentile10</dct:identifier>
        <rdfs:label xml:lang="en">NumericalDistribution - Percentile 10</rdfs:label>
        <vann:usageNote xml:lang="en">Optional property. This property can be used describe the 10th percentile of a collection of numbers.</vann:usageNote>
        <rdfs:comment xml:lang="en">The 10th percentile of a collection of numbers.</rdfs:comment>
    </owl:DatatypeProperty>

<!-- http://stelar-project.eu/klms#percentile25 -->
    <owl:DatatypeProperty rdf:about="http://stelar-project.eu/klms#percentile25">
        <rdfs:domain rdf:resource="http://stelar-project.eu/klms#NumericalDistribution"/>
        <rdfs:range rdf:resource="http://www.w3.org/2001/XMLSchema#float"/>
        <dct:identifier>klms:percentile25</dct:identifier>
        <rdfs:label xml:lang="en">NumericalDistribution - Percentile 25</rdfs:label>
        <vann:usageNote xml:lang="en">Optional property. This property can be used describe the 25th percentile of a collection of numbers.</vann:usageNote>
        <rdfs:comment xml:lang="en">The 25th percentile of a collection of numbers.</rdfs:comment>
    </owl:DatatypeProperty>

<!-- http://stelar-project.eu/klms#percentile75 -->
    <owl:DatatypeProperty rdf:about="http://stelar-project.eu/klms#percentile75">
        <rdfs:domain rdf:resource="http://stelar-project.eu/klms#NumericalDistribution"/>
        <rdfs:range rdf:resource="http://www.w3.org/2001/XMLSchema#float"/>
        <dct:identifier>klms:percentile75</dct:identifier>
        <rdfs:label xml:lang="en">NumericalDistribution - Percentile 75</rdfs:label>
        <vann:usageNote xml:lang="en">Optional property. This property can be used describe the 75th percentile of a collection of numbers.</vann:usageNote>
        <rdfs:comment xml:lang="en">The 75th percentile of a collection of numbers.</rdfs:comment>
    </owl:DatatypeProperty>

<!-- http://stelar-project.eu/klms#percentile90 -->
    <owl:DatatypeProperty rdf:about="http://stelar-project.eu/klms#percentile90">
        <rdfs:domain rdf:resource="http://stelar-project.eu/klms#NumericalDistribution"/>
        <rdfs:range rdf:resource="http://www.w3.org/2001/XMLSchema#float"/>
        <dct:identifier>klms:percentile90</dct:identifier>
        <rdfs:label xml:lang="en">NumericalDistribution - Percentile 90</rdfs:label>
        <vann:usageNote xml:lang="en">Optional property. This property can be used describe the 90th percentile of a collection of numbers.</vann:usageNote>
        <rdfs:comment xml:lang="en">The 90th percentile of a collection of numbers.</rdfs:comment>
    </owl:DatatypeProperty>




<!-- ####################################### -->
<!-- ##===================================## -->
<!-- ##==          CLASSES              ==## -->
<!-- ##===================================## --> 
<!-- ####################################### -->
    
<!-- ================================ -->
<!-- ==       MANDATORY CLASSES    == -->
<!-- ================================ -->

<!-- dcat:Dataset   -->
<!--
    <owl:Class rdf:about="http://www.w3.org/ns/dcat#Dataset">
    	<vann:usageNote xml:lang="en">Mandatory class. A conceptual entity that represents the information published.</vann:usageNote>
    	<dct:identifier>dcat:Dataset</dct:identifier>
    	<rdfs:label xml:lang="en">Dataset</rdfs:label>
        <rdfs:isDefinedBy rdf:resource="https://www.w3.org/TR/vocab-dcat-2/#Class:Dataset"/>
        <rdfs:comment xml:lang="en">A collection of data, published or curated by a single source, and available for access or download in one or more formats</rdfs:comment>
    </owl:Class>
-->

<!-- ================================ -->
<!-- ==     RECOMMENDED CLASSES    == -->
<!-- ================================ -->


<!-- dcat:Distribution -->
<!--
    <owl:Class rdf:about="http://www.w3.org/ns/dcat#Distribution">
    	<vann:usageNote xml:lang="en">Recommended class. A physical embodiment of the Dataset in a particular format.</vann:usageNote>
    	<dct:identifier>dcat:Distribution</dct:identifier>
    	<rdfs:label xml:lang="en">Distribution</rdfs:label>
    	<rdfs:isDefinedBy rdf:resource="https://www.w3.org/TR/vocab-dcat-2/#Class:Distribution"/>
        <rdfs:comment xml:lang="en">Represents a specific available form of a dataset. Each dataset might be available in different forms, these forms might represent different formats of the dataset, different endpoints,... Examples of Distribution include a downloadable CSV file, an XLS file representing the dataset, an RSS feed…</rdfs:comment>
    </owl:Class>
-->

<!-- klms:Dataset   -->
    <owl:Class rdf:about="http://stelar-project.eu/klms#Dataset">
    	<vann:usageNote xml:lang="en">Optional class. A collection of data, published or curated by a single source, and available for access or download in one or more representations.</vann:usageNote>
    	<dct:identifier>klms:Dataset</dct:identifier>
		<rdfs:subClassOf rdf:resource="http://www.w3.org/ns/dcat#Dataset"/>
    	<rdfs:label xml:lang="en">Dataset</rdfs:label>
		<skos:scopeNote xml:lang="en">This class describes the conceptual dataset. One or more representations might be available, with differing schematic layouts and formats or serializations.</skos:scopeNote>
        <rdfs:comment xml:lang="en">A collection of data, published or curated by a single source, and available for access or download in one or more formats.</rdfs:comment>
        <rdfs:subClassOf>
            <owl:Restriction>
                <owl:onProperty rdf:resource="http://purl.org/dc/terms/identifier"/>
                <owl:qualifiedCardinality rdf:datatype="http://www.w3.org/2001/XMLSchema#nonNegativeInteger">1</owl:qualifiedCardinality>
                <owl:onDataRange rdf:resource="http://www.w3.org/2001/XMLSchema#string"/>
            </owl:Restriction>
        </rdfs:subClassOf>
		<rdfs:subClassOf>
            <owl:Restriction>
                <owl:onProperty rdf:resource="http://www.w3.org/ns/dcat#keyword"/>
                <owl:minQualifiedCardinality rdf:datatype="http://www.w3.org/2001/XMLSchema#nonNegativeInteger">1</owl:minQualifiedCardinality>
                <owl:onDataRange rdf:resource="http://www.w3.org/2001/XMLSchema#string"/>
            </owl:Restriction>
        </rdfs:subClassOf>
    </owl:Class>
	
<!-- klms:Distribution   -->
    <owl:Class rdf:about="http://stelar-project.eu/klms#Distribution">
        <vann:usageNote xml:lang="en">Optional class. A DataProfile associated to a Dataset published or curated by a single agent.</vann:usageNote>
        <dct:identifier>klms:Distribution</dct:identifier>
        <rdfs:label xml:lang="en">Distribution</rdfs:label>
        <rdfs:comment xml:lang="en">The profiling information extracted from a Distribution of a Dataset.</rdfs:comment>
        <vann:usageNote xml:lang="en">Optional class. The profiling information extracted from a Distribution of a Dataset.</vann:usageNote>
        <rdfs:subClassOf rdf:resource="http://www.w3.org/ns/dcat#Distribution"/>
    </owl:Class>
	
<!-- klms:Organization -->
    <owl:Class rdf:about="http://stelar-project.eu/klms#Organization">
        <vann:usageNote xml:lang="en">Recommended class. Represents an organization that publishes data assets in the Catalog.</vann:usageNote>
		<dct:identifier>klms:Organization</dct:identifier>
    	<rdfs:label xml:lang="en">Organization</rdfs:label>
    	<rdfs:subClassOf rdf:resource="http://xmlns.com/foaf/0.1/#term_Organization"/>
        <rdfs:comment xml:lang="en">Represents an organization that publishes data assets in the Catalog.</rdfs:comment>
    </owl:Class>

<!-- klms:User -->
    <owl:Class rdf:about="http://stelar-project.eu/klms#User">
        <vann:usageNote xml:lang="en">Recommended class. Represents a User that has access to the Catalog under a given role (admin, editor, member) in an Organization.</vann:usageNote>
		<dct:identifier>klms:User</dct:identifier>
    	<rdfs:label xml:lang="en">User</rdfs:label>
    	<rdfs:subClassOf rdf:resource="http://xmlns.com/foaf/0.1/#term_Person"/>
        <rdfs:comment xml:lang="en">Represents a User that has access to the Catalog under a given role (admin, editor, member) in an Organization.</rdfs:comment>
    </owl:Class>
	
<!-- org:Role -->
<!--
	<owl:Class rdf:about="http://www.w3.org/ns/org/Role">
		<vann:usageNote xml:lang="en">Recommended class. Denotes a role that a User can take in an Organization. NOTE: In DCAT anf ORG vocabularies, this is a subclass of skos:Concept.</vann:usageNote>
		<dct:identifier>org:Role</dct:identifier>
		<rdfs:label xml:lang="en">Role</rdfs:label>
		<rdfs:isDefinedBy rdf:resource="http://www.w3.org/ns/org"/>
		<rdfs:comment xml:lang="en">Denotes a role that a User can take in an Organization. NOTE: In DCAT anf ORG vocabularies, this is a subclass of skos:Concept.</rdfs:comment>
	</owl:Class>
-->
	
<!-- org:Membership -->
<!--
	<owl:Class rdf:about="http://www.w3.org/ns/org/Membership">
		<vann:usageNote xml:lang="en">Recommended class. Indicates the nature of an User's membership of an Organization. NOTE: Represents an n-ary relation between a User, an Organization and a Role.</vann:usageNote>
		<dct:identifier>org:Membership</dct:identifier>
		<rdfs:label xml:lang="en">Membership</rdfs:label>
		<rdfs:isDefinedBy rdf:resource="http://www.w3.org/ns/org"/>
		<rdfs:comment xml:lang="en">Indicates the nature of an User's membership of an Organization. NOTE: Represents an n-ary relation between a User, an Organization and a Role.</rdfs:comment>
	</owl:Class>
-->

	
<!-- ================================ -->
<!-- ==      OPTIONAL CLASSES      == -->
<!-- ================================ -->



 <!-- klms:Raster   -->
    <owl:Class rdf:about="http://stelar-project.eu/klms#Raster">
    	<vann:usageNote xml:lang="en">Optional class. A DataProfile associated to a Dataset published or curated by a single agent.</vann:usageNote>
    	<dct:identifier>klms:Raster</dct:identifier>
    	<rdfs:label xml:lang="en">Raster</rdfs:label>
        <rdfs:comment xml:lang="en">The profiling information extracted from a Distribution of Raster Dataset.</rdfs:comment>
        <vann:usageNote xml:lang="en">Optional class. The profiling information extracted from a Distribution of a Raster Dataset.</vann:usageNote>
		<rdfs:subClassOf rdf:resource="http://stelar-project.eu/klms#Distribution"/>
    </owl:Class>
	
 <!-- klms:Tabular   -->
    <owl:Class rdf:about="http://stelar-project.eu/klms#Tabular">
    	<vann:usageNote xml:lang="en">Optional class. A geospatial-aware profile associated to a Dataset published or curated by a single agent.</vann:usageNote>
    	<dct:identifier>klms:Tabular</dct:identifier>
    	<rdfs:label xml:lang="en">Tabular</rdfs:label>
        <rdfs:comment xml:lang="en">The profiling information extracted from a Distribution of a Tabular Dataset.</rdfs:comment>
        <vann:usageNote xml:lang="en">Optional class. The profiling information extracted from a Distribution of a Tabular Dataset.</vann:usageNote>
		<rdfs:subClassOf rdf:resource="http://stelar-project.eu/klms#Distribution"/>
    </owl:Class>
	
 <!-- klms:Hierarchical   -->
    <owl:Class rdf:about="http://stelar-project.eu/klms#Hierarchical">
    	<vann:usageNote xml:lang="en">Optional class. A textual-aware profile associated to a Dataset published or curated by a single agent.</vann:usageNote>
    	<dct:identifier>klms:Hierarchical</dct:identifier>
    	<rdfs:label xml:lang="en">Hierarchical</rdfs:label>
        <rdfs:comment xml:lang="en">The profiling information extracted from a Distribution of a Hierarchical Dataset.</rdfs:comment>
        <vann:usageNote xml:lang="en">Optional class. The profiling information extracted from a Distribution of a Hierarchical Dataset.</vann:usageNote>
		<rdfs:subClassOf rdf:resource="http://stelar-project.eu/klms#Distribution"/>
    </owl:Class>

<!-- klms:RDFGraph   -->
    <owl:Class rdf:about="http://stelar-project.eu/klms#RDFGraph">
        <vann:usageNote xml:lang="en">Optional class. Combined profile associated to the various texts of a Dataset published or curated by a single agent.</vann:usageNote>
        <dct:identifier>klms:RDFGraph</dct:identifier>
        <rdfs:label xml:lang="en">RDFGraph</rdfs:label>
        <rdfs:comment xml:lang="en">The profiling information extracted from a Distribution of a RDFGraph Dataset.</rdfs:comment>
        <vann:usageNote xml:lang="en">Optional class. The profiling information extracted from a Distribution of a RDFGraph Dataset.</vann:usageNote>
        <rdfs:subClassOf rdf:resource="http://stelar-project.eu/klms#Distribution"/>
    </owl:Class>

<!-- klms:Text   -->
    <owl:Class rdf:about="http://stelar-project.eu/klms#Text">
        <vann:usageNote xml:lang="en">Optional class. Profiles associated to the various texts of a Dataset published or curated by a single agent.</vann:usageNote>
        <dct:identifier>klms:Text</dct:identifier>
        <rdfs:label xml:lang="en">Text</rdfs:label>
        <rdfs:comment xml:lang="en">The profiling information extracted from a Distribution of a Text Dataset.</rdfs:comment>
        <vann:usageNote xml:lang="en">Optional class. The profiling information extracted from a Distribution of a Text Dataset.</vann:usageNote>
        <rdfs:subClassOf rdf:resource="http://stelar-project.eu/klms#Distribution"/>
    </owl:Class>

<!-- klms:Attribute   -->
    <owl:Class rdf:about="http://stelar-project.eu/klms#Attribute">
        <vann:usageNote xml:lang="en">Optional class. Profiles associated to the languages of various texts of a Dataset published or curated by a single agent.</vann:usageNote>
        <dct:identifier>klms:Attribute</dct:identifier>
        <rdfs:label xml:lang="en">Attribute</rdfs:label>
        <rdfs:comment xml:lang="en">The profiling information extracted from an Attribute of a dataset.</rdfs:comment>
        <vann:usageNote xml:lang="en">Optional class. The profiling information extracted from an Attribute of a dataset.</vann:usageNote>
        <rdfs:hasParent rdf:resource="http://stelar-project.eu/klms#Attribute"/>
    </owl:Class>

<!-- klms:NumericalDistribution   -->
    <owl:Class rdf:about="http://stelar-project.eu/klms#NumericalDistribution">
        <vann:usageNote xml:lang="en">Optional class. Profiles associated to the distinct terms of various texts of a Dataset published or curated by a single agent.</vann:usageNote>
        <dct:identifier>klms:NumericalDistribution</dct:identifier>
        <rdfs:label xml:lang="en">NumericalDistribution</rdfs:label>
        <rdfs:comment xml:lang="en">A class used to describe numerical distribution information.</rdfs:comment>
        <vann:usageNote xml:lang="en">Optional class. A class used to describe numerical distribution information.</vann:usageNote>
    </owl:Class>

 <!-- klms:CategoricalDistribution   -->
    <owl:Class rdf:about="http://stelar-project.eu/klms#CategoricalDistribution">
    	<vann:usageNote xml:lang="en">Optional class. Profiles of a time series Dataset published or curated by a single agent.</vann:usageNote>
    	<dct:identifier>klms:CategoricalDistribution</dct:identifier>
    	<rdfs:label xml:lang="en">CategoricalDistribution</rdfs:label>
        <rdfs:comment xml:lang="en">A class used to describe categorical distribution information.</rdfs:comment>
        <vann:usageNote xml:lang="en">Optional class. A class used to describe categorical distribution information.</vann:usageNote>
    </owl:Class>

<!-- klms:NumericalAttribute   -->
    <owl:Class rdf:about="http://stelar-project.eu/klms#NumericalAttribute">
        <vann:usageNote xml:lang="en">Optional class. Geospatial-aware profiles associated to the various raster images that consist a Dataset published or curated by a single agent.</vann:usageNote>
        <dct:identifier>klms:NumericalAttribute</dct:identifier>
        <rdfs:label xml:lang="en">NumericalAttribute</rdfs:label>
        <rdfs:comment xml:lang="en">The profiling information extracted from a numerical attribute of a dataset.</rdfs:comment>
        <vann:usageNote xml:lang="en">Optional class. The profiling information extracted from a numerical attribute of a dataset.</vann:usageNote>
        <rdfs:subClassOf rdf:resource="http://stelar-project.eu/klms#Attribute"/>
    </owl:Class>

<!-- klms:TextualAttribute   -->
    <owl:Class rdf:about="http://stelar-project.eu/klms#TextualAttribute">
        <vann:usageNote xml:lang="en">Optional class. Geospatial-aware profiles associated to the band of a raster image from a Dataset published or curated by a single agent.</vann:usageNote>
        <dct:identifier>klms:TextualAttribute</dct:identifier>
        <rdfs:label xml:lang="en">TextualAttribute</rdfs:label>
        <rdfs:comment xml:lang="en">The profiling information extracted from a textual attribute of a dataset.</rdfs:comment>
        <vann:usageNote xml:lang="en">Optional class. The profiling information extracted from a textual attribute of a dataset.</vann:usageNote>
        <rdfs:subClassOf rdf:resource="http://stelar-project.eu/klms#Attribute"/>
    </owl:Class>

<!-- klms:TemporalAttribute   -->
    <owl:Class rdf:about="http://stelar-project.eu/klms#TemporalAttribute">
        <vann:usageNote xml:lang="en">Optional class. Geospatial-aware profiles associated to an applied mask on a raster image from a Dataset published or curated by a single agent.</vann:usageNote>
        <dct:identifier>klms:TemporalAttribute</dct:identifier>
        <rdfs:label xml:lang="en">TemporalAttribute</rdfs:label>
        <rdfs:comment xml:lang="en">The profiling information extracted from a temporal attribute of a dataset.</rdfs:comment>
        <vann:usageNote xml:lang="en">Optional class. The profiling information extracted from a temporal attribute of a dataset.</vann:usageNote>
        <rdfs:subClassOf rdf:resource="http://stelar-project.eu/klms#Attribute"/>
    </owl:Class>    

<!-- klms:SpatialAttribute   -->
    <owl:Class rdf:about="http://stelar-project.eu/klms#SpatialAttribute">
        <vann:usageNote xml:lang="en">Optional class. Geospatial-aware profiles associated to an applied mask on a raster image from a Dataset published or curated by a single agent.</vann:usageNote>
        <dct:identifier>klms:SpatialAttribute</dct:identifier>
        <rdfs:label xml:lang="en">SpatialAttribute</rdfs:label>
        <rdfs:comment xml:lang="en">The profiling information extracted from a spatial attribute of a dataset.</rdfs:comment>
        <vann:usageNote xml:lang="en">Optional class. The profiling information extracted from a spatial attribute of a dataset.</vann:usageNote>
        <rdfs:subClassOf rdf:resource="http://stelar-project.eu/klms#Attribute"/>
    </owl:Class>

<!-- klms:CategoricalAttribute   -->
    <owl:Class rdf:about="http://stelar-project.eu/klms#CategoricalAttribute">
        <vann:usageNote xml:lang="en">Optional class. Geospatial-aware profiles associated to an applied mask on a raster image from a Dataset published or curated by a single agent.</vann:usageNote>
        <dct:identifier>klms:CategoricalAttribute</dct:identifier>
        <rdfs:label xml:lang="en">CategoricalAttribute</rdfs:label>
        <rdfs:comment xml:lang="en">The profiling information extracted from a categorical attribute of a dataset.</rdfs:comment>
        <vann:usageNote xml:lang="en">Optional class. The profiling information extracted from a categorical attribute of a dataset.</vann:usageNote>
        <rdfs:subClassOf rdf:resource="http://stelar-project.eu/klms#Attribute"/>
    </owl:Class>

<!-- klms:SeriesAttribute   -->
    <owl:Class rdf:about="http://stelar-project.eu/klms#SeriesAttribute">
        <vann:usageNote xml:lang="en">Optional class. Geospatial-aware profiles associated to an applied mask on a raster image from a Dataset published or curated by a single agent.</vann:usageNote>
        <dct:identifier>klms:SeriesAttribute</dct:identifier>
        <rdfs:label xml:lang="en">SeriesAttribute</rdfs:label>
        <rdfs:comment xml:lang="en">The profiling information extracted from a series attribute of a dataset.</rdfs:comment>
        <vann:usageNote xml:lang="en">Optional class. The profiling information extracted from a series attribute of a dataset.</vann:usageNote>
        <rdfs:subClassOf rdf:resource="http://stelar-project.eu/klms#NumericalAttribute"/>
    </owl:Class>

<!-- klms:BandAttribute 
    <owl:Class rdf:about="http://stelar-project.eu/klms#BandAttribute">
        <vann:usageNote xml:lang="en">Optional class. Geospatial-aware profiles associated to an applied mask on a raster image from a Dataset published or curated by a single agent.</vann:usageNote>
        <dct:identifier>klms:BandAttribute</dct:identifier>
        <rdfs:label xml:lang="en">BandAttribute</rdfs:label>
        <rdfs:comment xml:lang="en">The profiling information extracted from a band attribute of a dataset.</rdfs:comment>
        <vann:usageNote xml:lang="en">Optional class. The profiling information extracted from a band attribute of a dataset.</vann:usageNote>
        <rdfs:subClassOf rdf:resource="http://stelar-project.eu/klms#NumericalAttribute"/>
    </owl:Class>
-->

<!-- klms:Category   -->
    <owl:Class rdf:about="http://stelar-project.eu/klms#Category">
        <vann:usageNote xml:lang="en">Optional class. Geospatial-aware profiles associated to an applied mask on a raster image from a Dataset published or curated by a single agent.</vann:usageNote>
        <dct:identifier>klms:Category</dct:identifier>
        <rdfs:label xml:lang="en">Category</rdfs:label>
        <rdfs:comment xml:lang="en">A class representing a category of a categorical distribution.</rdfs:comment>
        <vann:usageNote xml:lang="en">Optional class. A class representing a category of a categorical distribution.</vann:usageNote>
        <rdfs:subClassOf rdf:resource="http://stelar-project.eu/klms#CategoricalDistribution"/>
    </owl:Class>

<!-- klms:KeyValuePair -->
    <owl:Class rdf:about="http://stelar-project.eu/klms#KeyValuePair">
		<vann:usageNote xml:lang="en">Optional class. An extra (custom) metadata item represented as a key/value pair.</vann:usageNote>
    	<dct:identifier>klms:KeyValuePair</dct:identifier>
    	<rdfs:label xml:lang="en">KeyValuePair</rdfs:label>
		<rdfs:comment xml:lang="en">An extra (custom) metadata item of a Dataset represented as a key/value pair.</rdfs:comment>
        <rdfs:subClassOf>
            <owl:Restriction>
                <owl:onProperty rdf:resource="http://stelar-project.eu/klms#key"/>
                <owl:qualifiedCardinality rdf:datatype="http://www.w3.org/2001/XMLSchema#nonNegativeInteger">1</owl:qualifiedCardinality>
                <owl:onDataRange rdf:resource="http://www.w3.org/2001/XMLSchema#string"/>
            </owl:Restriction>
        </rdfs:subClassOf>
        <rdfs:subClassOf>
            <owl:Restriction>
                <owl:onProperty rdf:resource="http://stelar-project.eu/klms#value"/>
                <owl:qualifiedCardinality rdf:datatype="http://www.w3.org/2001/XMLSchema#nonNegativeInteger">1</owl:qualifiedCardinality>
                <owl:onDataRange rdf:resource="http://www.w3.org/1999/02/22-rdf-syntax-ns#PlainLiteral"/>
            </owl:Restriction>
        </rdfs:subClassOf>
        <rdfs:comment xml:lang="en">An extra (custom) metadata item represented as a key/value pair.</rdfs:comment>
    </owl:Class>

 <!-- klms:Workflow   -->
    <owl:Class rdf:about="http://stelar-project.eu/klms#Workflow">
    	<vann:usageNote xml:lang="en">Recommended class. A workflow defined by a User and involving at least one task.</vann:usageNote>
    	<dct:identifier>klms:Workflow</dct:identifier>
    	<rdfs:label xml:lang="en">Workflow</rdfs:label>
        <rdfs:comment xml:lang="en">A workflow defined by a User and involving at least one task. It can be invoked ad-hoc by a user or scheduled to run (e.g., hourly, daily, etc.), each resulting in an instance of WorkflowExecution.</rdfs:comment>
    </owl:Class>

 <!-- klms:WorkflowExecution   -->
    <owl:Class rdf:about="http://stelar-project.eu/klms#WorkflowExecution">
    	<vann:usageNote xml:lang="en">Recommended class. An instance of a workflow defined by a User.</vann:usageNote>
    	<dct:identifier>klms:WorkflowExecution</dct:identifier>
    	<rdfs:label xml:lang="en">WorkflowExecution</rdfs:label>
        <rdfs:comment xml:lang="en">An instance of a workflow defined by a User. .</rdfs:comment>
    </owl:Class>
	
 <!-- klms:Task   -->
    <owl:Class rdf:about="http://stelar-project.eu/klms#Task">
    	<vann:usageNote xml:lang="en">Recommended class. A task respresent a processing job that takes some input and produces some output within a workflow.</vann:usageNote>
    	<dct:identifier>klms:Task</dct:identifier>
    	<rdfs:label xml:lang="en">Task</rdfs:label>
        <rdfs:comment xml:lang="en">A task respresent a processing job that takes some input and produces some output within a workflow. An instance of a WorkflowExecution creates a new instance of this task.</rdfs:comment>
    </owl:Class>
	
 <!-- klms:TaskExecution   -->
    <owl:Class rdf:about="http://stelar-project.eu/klms#TaskExecution">
    	<vann:usageNote xml:lang="en">Recommended class. An instance of a task running within a workflow execution.</vann:usageNote>
    	<dct:identifier>klms:TaskExecution</dct:identifier>
    	<rdfs:label xml:lang="en">TaskExecution</rdfs:label>
        <rdfs:comment xml:lang="en">An instance of a task running within a workflow execution. Parameters, tags, and metrics are recorded for each task execution.</rdfs:comment>
    </owl:Class>
	
	
<!-- ################################################# -->
<!-- ##=============================================## -->
<!-- ##==          OBJECT PROPERTIES              ==## -->
<!-- ##=============================================## --> 
<!-- ################################################# -->
 
<!--  Attribute - contains  -->
    <owl:ObjectProperty rdf:about="http://stelar-project.eu/klms#contains">
		<rdfs:label xml:lang="en">Contains</rdfs:label>
        <dct:identifier>klms:contains</dct:identifier>
        <vann:usageNote xml:lang="en">Optional property. This property is used to indicate a contains relation among classes.</vann:usageNote>
        <rdfs:comment xml:lang="en">This property is used to indicate a contains relation among classes.</rdfs:comment>
    </owl:ObjectProperty>

<!--  NumericalDistribution - depth distribution  -->
    <owl:ObjectProperty rdf:about="http://stelar-project.eu/klms#depthDistribution">
        <rdfs:label xml:lang="en">NumericalDistribution - Depth distribution</rdfs:label>
        <rdfs:domain rdf:resource="http://stelar-project.eu/klms#Hierarchical"/>
        <rdfs:range rdf:resource="http://stelar-project.eu/klms#NumericalDistribution"/>
        <dct:identifier>klms:depthDistribution</dct:identifier>
        <vann:usageNote xml:lang="en">Optional property. This property is used to indicate the depth distribution of a hierarchical dataset.</vann:usageNote>
        <rdfs:comment xml:lang="en">This property is used to indicate the depth distribution of a hierarchical dataset.</rdfs:comment>
    </owl:ObjectProperty>
    
<!--  NumericalDistribution - degree distribution  -->
    <owl:ObjectProperty rdf:about="http://stelar-project.eu/klms#degreeDistribution">
        <rdfs:label xml:lang="en">NumericalDistribution - Degree distribution</rdfs:label>
        <rdfs:domain rdf:resource="http://stelar-project.eu/klms#RDFGraph"/>
        <rdfs:range rdf:resource="http://stelar-project.eu/klms#NumericalDistribution"/>
        <dct:identifier>klms:degreeDistribution</dct:identifier>
        <vann:usageNote xml:lang="en">Optional property. This property is used to indicate the degree distribution of an RDF graph.</vann:usageNote>
        <rdfs:comment xml:lang="en">This property is used to indicate the degree distribution of an RDF graph.</rdfs:comment>
    </owl:ObjectProperty>

<!--  NumericalDistribution - class distribution  -->
    <owl:ObjectProperty rdf:about="http://stelar-project.eu/klms#classDistribution">
        <rdfs:label xml:lang="en">CategoricalDistribution - Class distribution</rdfs:label>
        <rdfs:domain rdf:resource="http://stelar-project.eu/klms#RDFGraph"/>
        <rdfs:range rdf:resource="http://stelar-project.eu/klms#CategoricalDistribution"/>
        <dct:identifier>klms:classDistribution</dct:identifier>
        <vann:usageNote xml:lang="en">Optional property. This property is used to indicate the class distribution of an RDF graph.</vann:usageNote>
        <rdfs:comment xml:lang="en">This property is used to indicate the class distribution of an RDF graph.</rdfs:comment>
    </owl:ObjectProperty>
    
<!--  NumericalDistribution - sentence length distribution  -->
    <owl:ObjectProperty rdf:about="http://stelar-project.eu/klms#sentenceLengthDistribution">
        <rdfs:label xml:lang="en">NumericalDistribution - Sentence length distribution</rdfs:label>
        <rdfs:domain rdf:resource="http://stelar-project.eu/klms#Text"/>
        <rdfs:range rdf:resource="http://stelar-project.eu/klms#NumericalDistribution"/>
        <dct:identifier>klms:sentenceLengthDistribution</dct:identifier>
        <vann:usageNote xml:lang="en">Optional property. This property is used to indicate the sentence length distribution of a text.</vann:usageNote>
        <rdfs:comment xml:lang="en">This property is used to indicate the sentence length distribution of a text.</rdfs:comment>
    </owl:ObjectProperty>

<!--  NumericalDistribution - word length distribution  -->
    <owl:ObjectProperty rdf:about="http://stelar-project.eu/klms#wordLengthDistribution">
        <rdfs:label xml:lang="en">NumericalDistribution - Word length distribution</rdfs:label>
        <rdfs:domain rdf:resource="http://stelar-project.eu/klms#Text"/>
        <rdfs:range rdf:resource="http://stelar-project.eu/klms#NumericalDistribution"/>
        <dct:identifier>klms:wordLengthDistribution</dct:identifier>
        <vann:usageNote xml:lang="en">Optional property. This property is used to indicate the word length distribution of a text.</vann:usageNote>
        <rdfs:comment xml:lang="en">This property is used to indicate the word length distribution of a text.</rdfs:comment>
    </owl:ObjectProperty>

<!--  NumericalDistribution - language distribution  -->
    <owl:ObjectProperty rdf:about="http://stelar-project.eu/klms#languageDistribution">
        <rdfs:label xml:lang="en">CategoricalDistribution - Language distribution</rdfs:label>
        <rdfs:domain rdf:resource="http://stelar-project.eu/klms#Text"/>
        <rdfs:range rdf:resource="http://stelar-project.eu/klms#CategoricalDistribution"/>
        <dct:identifier>klms:languageDistribution</dct:identifier>
        <vann:usageNote xml:lang="en">Optional property. This property is used to indicate the language distribution of a text.</vann:usageNote>
        <rdfs:comment xml:lang="en">This property is used to indicate the language distribution of a text.</rdfs:comment>
    </owl:ObjectProperty>

<!--  NumericalDistribution - special characters distribution  -->
    <owl:ObjectProperty rdf:about="http://stelar-project.eu/klms#specialCharsDistribution">
        <rdfs:label xml:lang="en">CategoricalDistribution - Special characters distribution</rdfs:label>
        <rdfs:domain rdf:resource="http://stelar-project.eu/klms#Text"/>
        <rdfs:range rdf:resource="http://stelar-project.eu/klms#CategoricalDistribution"/>
        <dct:identifier>klms:specialCharsDistribution</dct:identifier>
        <vann:usageNote xml:lang="en">Optional property. This property is used to indicate the special characters distribution of a text.</vann:usageNote>
        <rdfs:comment xml:lang="en">This property is used to indicate the special characters distribution of a text.</rdfs:comment>
    </owl:ObjectProperty>

<!--  Numerical distribution - value distribution  -->
    <owl:ObjectProperty rdf:about="http://stelar-project.eu/klms#valueDistribution">
        <rdfs:label xml:lang="en">NumericalDistribution - Value distribution</rdfs:label>
        <rdfs:domain rdf:resource="http://stelar-project.eu/klms#NumericalAttribute"/>
        <rdfs:range rdf:resource="http://stelar-project.eu/klms#NumericalDistribution"/>
        <dct:identifier>klms:valueDistribution</dct:identifier>
        <vann:usageNote xml:lang="en">Optional property. This property is used to indicate the value distribution of a numerical attribute.</vann:usageNote>
        <rdfs:comment xml:lang="en">This property is used to indicate the value distribution of a numerical attribute.</rdfs:comment>
    </owl:ObjectProperty>

<!--  Numerical distribution - number of characters distribution  -->
    <owl:ObjectProperty rdf:about="http://stelar-project.eu/klms#numCharsDistribution">
        <rdfs:label xml:lang="en">NumericalDistribution - Number of characters distribution</rdfs:label>
        <rdfs:domain rdf:resource="http://stelar-project.eu/klms#TextualAttribute"/>
        <rdfs:range rdf:resource="http://stelar-project.eu/klms#NumericalDistribution"/>
        <dct:identifier>klms:numCharsDistribution</dct:identifier>
        <vann:usageNote xml:lang="en">Optional property. This property is used to indicate the number of characters distribution of a textual attribute.</vann:usageNote>
        <rdfs:comment xml:lang="en">This property is used to indicate the number of characters distribution of a textual attribute.</rdfs:comment>
    </owl:ObjectProperty>
    
<!--  Numerical distribution - number of words distribution  -->
    <owl:ObjectProperty rdf:about="http://stelar-project.eu/klms#numWordsDistribution">
        <rdfs:label xml:lang="en">NumericalDistribution - Number of words distribution</rdfs:label>
        <rdfs:domain rdf:resource="http://stelar-project.eu/klms#TextualAttribute"/>
        <rdfs:range rdf:resource="http://stelar-project.eu/klms#NumericalDistribution"/>
        <dct:identifier>klms:numWordsDistribution</dct:identifier>
        <vann:usageNote xml:lang="en">Optional property. This property is used to indicate the number of words distribution of a textual attribute.</vann:usageNote>
        <rdfs:comment xml:lang="en">This property is used to indicate the number of words distribution of a textual attribute.</rdfs:comment>
    </owl:ObjectProperty>

<!--  Numerical distribution - resolution distribution  -->
    <owl:ObjectProperty rdf:about="http://stelar-project.eu/klms#resolutionDistribution">
        <rdfs:label xml:lang="en">NumericalDistribution - Resolution distribution</rdfs:label>
        <rdfs:domain rdf:resource="http://stelar-project.eu/klms#TemporalAttribute"/>
        <rdfs:range rdf:resource="http://stelar-project.eu/klms#NumericalDistribution"/>
        <dct:identifier>klms:resolutionDistribution</dct:identifier>
        <vann:usageNote xml:lang="en">Optional property. This property is used to indicate the resolution distribution of a temporal attribute.</vann:usageNote>
        <rdfs:comment xml:lang="en">This property is used to indicate the resolution distribution of a temporal attribute.</rdfs:comment>
    </owl:ObjectProperty>

<!--  Numerical distribution - length distribution  -->
    <owl:ObjectProperty rdf:about="http://stelar-project.eu/klms#lengthDistribution">
        <rdfs:label xml:lang="en">NumericalDistribution - Length distribution</rdfs:label>
        <rdfs:domain rdf:resource="http://stelar-project.eu/klms#SpatialAttribute"/>
        <rdfs:range rdf:resource="http://stelar-project.eu/klms#NumericalDistribution"/>
        <dct:identifier>klms:lengthDistribution</dct:identifier>
        <vann:usageNote xml:lang="en">Optional property. This property is used to indicate the geometry length distribution of a spatial attribute.</vann:usageNote>
        <rdfs:comment xml:lang="en">This property is used to indicate the geometry length distribution of a spatial attribute.</rdfs:comment>
    </owl:ObjectProperty>

<!--  Numerical distribution - area distribution  -->
    <owl:ObjectProperty rdf:about="http://stelar-project.eu/klms#areaDistribution">
        <rdfs:label xml:lang="en">NumericalDistribution - Area distribution</rdfs:label>
        <rdfs:domain rdf:resource="http://stelar-project.eu/klms#SpatialAttribute"/>
        <rdfs:range rdf:resource="http://stelar-project.eu/klms#NumericalDistribution"/>
        <dct:identifier>klms:areaDistribution</dct:identifier>
        <vann:usageNote xml:lang="en">Optional property. This property is used to indicate the geometry area distribution of a spatial attribute.</vann:usageNote>
        <rdfs:comment xml:lang="en">This property is used to indicate the geometry area distribution of a spatial attribute.</rdfs:comment>
    </owl:ObjectProperty>

<!--  Categorical distribution - geometry type distribution  -->
    <owl:ObjectProperty rdf:about="http://stelar-project.eu/klms#geomTypeDistribution">
        <rdfs:label xml:lang="en">NumericalDistribution - Geometry type distribution</rdfs:label>
        <rdfs:domain rdf:resource="http://stelar-project.eu/klms#SpatialAttribute"/>
        <rdfs:range rdf:resource="http://stelar-project.eu/klms#CategoricalDistribution"/>
        <dct:identifier>klms:geomTypeDistribution</dct:identifier>
        <vann:usageNote xml:lang="en">Optional property. This property is used to indicate the geometry type distribution of a spatial attribute.</vann:usageNote>
        <rdfs:comment xml:lang="en">This property is used to indicate the geometry type distribution of a spatial attribute.</rdfs:comment>
    </owl:ObjectProperty>

<!--  Categorical distribution - frequency distribution  -->
    <owl:ObjectProperty rdf:about="http://stelar-project.eu/klms#frequencyDistribution">
        <rdfs:label xml:lang="en">NumericalDistribution - Frequency distribution</rdfs:label>
        <rdfs:domain rdf:resource="http://stelar-project.eu/klms#CategoricalAttribute"/>
        <rdfs:range rdf:resource="http://stelar-project.eu/klms#CategoricalDistribution"/>
        <dct:identifier>klms:frequencyDistribution</dct:identifier>
        <vann:usageNote xml:lang="en">Optional property. This property is used to indicate the frequency distribution of a categorical attribute.</vann:usageNote>
        <rdfs:comment xml:lang="en">This property is used to indicate the frequency distribution of a categorical attribute.</rdfs:comment>
    </owl:ObjectProperty>


 <!--  Workflow - creator  -->
	 <owl:ObjectProperty rdf:about="http://purl.org/dc/terms/creator"> 
		  <vann:usageNote xml:lang="en">Optional property. This property refers to the User that created this Workflow.</vann:usageNote>
		  <dct:identifier>dct:creator</dct:identifier>
		  <rdfs:domain rdf:resource="http://stelar-project.eu/klms#Workflow"/>
		  <rdfs:range rdf:resource="http://stelar-project.eu/klms#User"/>
		  <rdfs:label xml:lang="en">Workflow - creator</rdfs:label>
		  <rdfs:comment xml:lang="en">This property refers to the User that created this Workflow.</rdfs:comment>
	 </owl:ObjectProperty>

 <!--  Workflow - hasParent  -->
	 <owl:ObjectProperty rdf:about="http://stelar-project.eu/klms#hasParent"> 
		  <vann:usageNote xml:lang="en">Optional property. This property indicates the Workflow that spawned the current Workflow.</vann:usageNote>
		  <dct:identifier>klms:hasParent</dct:identifier>
		  <rdfs:domain rdf:resource="http://stelar-project.eu/klms#Workflow"/>
		  <rdfs:range rdf:resource="http://stelar-project.eu/klms#Workflow"/>
		  <rdfs:label xml:lang="en">Workflow - hasParent</rdfs:label>
		  <rdfs:comment xml:lang="en">This property indicates the Workflow that spawned (is parent of) the current Workflow.</rdfs:comment>
	 </owl:ObjectProperty>
	 
 <!--  Workflow - description  -->
	 <owl:DatatypeProperty rdf:about="http://purl.org/dc/terms/description"> 
		  <vann:usageNote xml:lang="en">Recommended property. This property contains a free-text description of the Workflow.</vann:usageNote>
		  <dct:identifier>dct:description</dct:identifier>
		  <rdfs:domain rdf:resource="http://stelar-project.eu/klms#Workflow"/>
		  <rdfs:range rdf:resource="http://www.w3.org/2000/01/rdf-schema#Literal"/>
		  <rdfs:label xml:lang="en">Workflow - description</rdfs:label>
		  <rdfs:comment xml:lang="en">This property contains a free-text description of the Workflow.</rdfs:comment>
	 </owl:DatatypeProperty>
 
<!--  Workflow - title  -->
	 <owl:DatatypeProperty rdf:about="http://purl.org/dc/terms/title"> 
		  <vann:usageNote xml:lang="en">Recommended property. This property contains a name given to the Workflow.</vann:usageNote>
		  <dct:identifier>dct:title</dct:identifier>
		  <rdfs:domain rdf:resource="http://stelar-project.eu/klms#Workflow"/>
		  <rdfs:range rdf:resource="http://www.w3.org/2000/01/rdf-schema#Literal"/>
		  <rdfs:label xml:lang="en">Workflow - title</rdfs:label>
		  <rdfs:comment xml:lang="en">This property contains a name (title) given to the Workflow.</rdfs:comment>
	 </owl:DatatypeProperty>

<!--  Workflow - schedule  -->
	 <owl:DatatypeProperty rdf:about="http://stelar-project.eu/klms#schedule"> 
		  <vann:usageNote xml:lang="en">Optional property. This property denotes the schedule interval (e.g., hourly, daily) for executing this Workflow.</vann:usageNote>
		  <dct:identifier>klms:schedule</dct:identifier>
		  <rdfs:domain rdf:resource="http://stelar-project.eu/klms#Workflow"/>
		  <rdfs:range rdf:resource="http://www.w3.org/2000/01/rdf-schema#Literal"/>
		  <rdfs:label xml:lang="en">Workflow - schedule</rdfs:label>
		  <rdfs:comment xml:lang="en">This property denotes the schedule interval (e.g., hourly, daily) for executing this Workflow.</rdfs:comment>
	 </owl:DatatypeProperty>
	 
<!--  Workflow - nextRun  -->
	 <owl:DatatypeProperty rdf:about="http://stelar-project.eu/klms#nextRun"> 
		  <vann:usageNote xml:lang="en">Optional property. This property denotes the next time when the Workflow is scheduled to run again.</vann:usageNote>
		  <dct:identifier>klms:nextRun</dct:identifier>
		  <rdfs:domain rdf:resource="http://stelar-project.eu/klms#Workflow"/>
		  <rdfs:range rdf:resource="http://www.w3.org/2001/XMLSchema#dateTime"/>
		  <rdfs:label xml:lang="en">Workflow - nextRun</rdfs:label>
		  <rdfs:comment xml:lang="en">This property denotes the next time when the Workflow is scheduled to run again.</rdfs:comment>
	 </owl:DatatypeProperty>
	 
 <!--  WorkflowExecution - instantiates -->
	 <rdf:ObjectProperty rdf:about="http://stelar-project.eu/klms#instantiates"> 
		  <vann:usageNote xml:lang="en">Recommended property. This property denotes that a WorkflowExecution is an instance of Workflow.</vann:usageNote>
		  <dct:identifier>klms:instantiates</dct:identifier>
		  <rdfs:label xml:lang="en">WorkflowExecution - instantiates</rdfs:label>
		  <rdfs:domain rdf:resource="http://stelar-project.eu/klms#WorkflowExecution"/>
		  <rdfs:range rdf:resource="http://stelar-project.eu/klms#Workflow"/>
		  <rdfs:comment xml:lang="en">This property denotes that a WorkflowExecution is an instance of a Workflow.</rdfs:comment>
	 </rdf:ObjectProperty>

 <!--  WorkflowExecution - state -->
	 <rdf:DatatypeProperty rdf:about="http://stelar-project.eu/klms#state"> 
		  <vann:usageNote xml:lang="en">Recommended property. This property denotes the current state of a WorkflowExecution.</vann:usageNote>
		  <dct:identifier>klms:state</dct:identifier>
		  <rdfs:label xml:lang="en">WorkflowExecution - state</rdfs:label>
		  <rdfs:domain rdf:resource="http://stelar-project.eu/klms#WorkflowExecution"/>
		  <rdfs:range rdf:resource="http://www.w3.org/2000/01/rdf-schema#Literal"/>
		  <rdfs:comment xml:lang="en">This property denotes the current state of a WorkflowExecution.</rdfs:comment>
	 </rdf:DatatypeProperty>
	 
<!--  WorkflowExecution - start date  -->
	 <owl:DatatypeProperty rdf:about="http://www.w3.org/ns/dcat#startDate"> 
		  <vann:usageNote xml:lang="en">Optional property. This property denotes the starting time of a WorkflowExecution.</vann:usageNote>
		  <dct:identifier>dcat:startDate</dct:identifier>
		  <rdfs:domain rdf:resource="http://stelar-project.eu/klms#WorkflowExecution"/>
		  <rdfs:range rdf:resource="http://www.w3.org/2001/XMLSchema#dateTime"/>
		  <rdfs:label xml:lang="en">WorkflowExecution - start date</rdfs:label>
	  <rdfs:comment xml:lang="en">This property denotes the starting time of a WorkflowExecution.</rdfs:comment>
	 </owl:DatatypeProperty>
 
<!--  WorkflowExecution - end date  -->
	 <owl:DatatypeProperty rdf:about="http://www.w3.org/ns/dcat#endDate"> 
		  <vann:usageNote xml:lang="en">Optional property. This property contains the end time of a WorkflowExecution.</vann:usageNote>
		  <dct:identifier>dcat:endDate</dct:identifier>
		  <rdfs:domain rdf:resource="http://stelar-project.eu/klms#WorkflowExecution"/>
		  <rdfs:range rdf:resource="http://www.w3.org/2001/XMLSchema#dateTime"/>
		  <rdfs:label xml:lang="en">WorkflowExecution - end date</rdfs:label>
		  <rdfs:comment xml:lang="en">This property denotes the end time of a WorkflowExecution.</rdfs:comment>
	 </owl:DatatypeProperty>

<!--  Task - isPartOf  -->
	 <rdf:ObjectProperty rdf:about="http://purl.org/dc/terms/isPartOf"> 
		  <vann:usageNote xml:lang="en">Recommended property. This property refers to a Task that is involved in a Workflow.</vann:usageNote>
		  <dct:identifier>dct:isPartOf</dct:identifier>
		  <rdfs:label xml:lang="en">Task - is part of</rdfs:label>
		  <rdfs:domain rdf:resource="http://stelar-project.eu/klms#Task"/>
		  <rdfs:range rdf:resource="http://stelar-project.eu/klms#Workflow"/>
		  <rdfs:isDefinedBy rdf:resource="http://dublincore.org/documents/dcmi-terms/#terms-isPartOf" />
		  <rdfs:comment xml:lang="en">This property refers to a Task that is involved in a Workflow.</rdfs:comment>
	 </rdf:ObjectProperty>
	 
<!--  Task - title  -->
	 <owl:DatatypeProperty rdf:about="http://purl.org/dc/terms/title"> 
		  <vann:usageNote xml:lang="en">Recommended property. This property contains a name given to the Task.</vann:usageNote>
		  <dct:identifier>dct:title</dct:identifier>
		  <rdfs:domain rdf:resource="http://stelar-project.eu/klms#Task"/>
		  <rdfs:range rdf:resource="http://www.w3.org/2000/01/rdf-schema#Literal"/>
		  <rdfs:label xml:lang="en">Task - title</rdfs:label>
		  <rdfs:comment xml:lang="en">This property contains a name (title) given to the Task.</rdfs:comment>
	 </owl:DatatypeProperty>

<!--  TaskExecution - instantiates -->
	 <rdf:ObjectProperty rdf:about="http://stelar-project.eu/klms#instantiates"> 
		  <vann:usageNote xml:lang="en">Recommended property. This property denotes that a TaskExecution is an instance of a Task defined in a Workflow.</vann:usageNote>
		  <dct:identifier>klms:instantiates</dct:identifier>
		  <rdfs:label xml:lang="en">TaskExecution - instantiates</rdfs:label>
		  <rdfs:domain rdf:resource="http://stelar-project.eu/klms#TaskExecution"/>
		  <rdfs:range rdf:resource="http://stelar-project.eu/klms#Task"/>
		  <rdfs:comment xml:lang="en">This property denotes that a TaskExecution is an instance of a Task defined in a Workflow.</rdfs:comment>
	 </rdf:ObjectProperty>

<!--  TaskExecution - isPartOf  -->
	 <rdf:ObjectProperty rdf:about="http://purl.org/dc/terms/isPartOf"> 
		  <vann:usageNote xml:lang="en">Recommended property. This property refers to a TaskExecution that is involved in a WorkflowExecution.</vann:usageNote>
		  <dct:identifier>dct:isPartOf</dct:identifier>
		  <rdfs:label xml:lang="en">TaskExecution - is part of</rdfs:label>
		  <rdfs:domain rdf:resource="http://stelar-project.eu/klms#TaskExecution"/>
		  <rdfs:range rdf:resource="http://stelar-project.eu/klms#WorkflowExecution"/>
		  <rdfs:isDefinedBy rdf:resource="http://dublincore.org/documents/dcmi-terms/#terms-isPartOf" />
		  <rdfs:comment xml:lang="en">This property refers to a TaskExecution that is involved in a WorkflowExecution.</rdfs:comment>
	 </rdf:ObjectProperty>

 <!--  TaskExecution - state -->
	 <rdf:ObjectProperty rdf:about="http://stelar-project.eu/klms#state"> 
		  <vann:usageNote xml:lang="en">Recommended property. This property denotes the current state of a TaskExecution.</vann:usageNote>
		  <dct:identifier>klms:state</dct:identifier>
		  <rdfs:label xml:lang="en">TaskExecution - state</rdfs:label>
		  <rdfs:domain rdf:resource="http://stelar-project.eu/klms#TaskExecution"/>
		  <rdfs:range rdf:resource="http://www.w3.org/2000/01/rdf-schema#Literal"/>
		  <rdfs:comment xml:lang="en">This property denotes the current state of a TaskExecution.</rdfs:comment>
	 </rdf:ObjectProperty>
	 
<!--  TaskExecution - start date  -->
	 <owl:DatatypeProperty rdf:about="http://www.w3.org/ns/dcat#startDate"> 
		  <vann:usageNote xml:lang="en">Optional property. This property denotes the starting time of a TaskExecution.</vann:usageNote>
		  <dct:identifier>dcat:startDate</dct:identifier>
		  <rdfs:domain rdf:resource="http://stelar-project.eu/klms#TaskExecution"/>
		  <rdfs:range rdf:resource="http://www.w3.org/2001/XMLSchema#dateTime"/>
		  <rdfs:label xml:lang="en">TaskExecution - start date</rdfs:label>
	  <rdfs:comment xml:lang="en">This property denotes the starting time of a TaskExecution.</rdfs:comment>
	 </owl:DatatypeProperty>
 
<!--  TaskExecution - end date  -->
	 <owl:DatatypeProperty rdf:about="http://www.w3.org/ns/dcat#endDate"> 
		  <vann:usageNote xml:lang="en">Optional property. This property contains the end time of a TaskExecution.</vann:usageNote>
		  <dct:identifier>dcat:endDate</dct:identifier>
		  <rdfs:domain rdf:resource="http://stelar-project.eu/klms#TaskExecution"/>
		  <rdfs:range rdf:resource="http://www.w3.org/2001/XMLSchema#dateTime"/>
		  <rdfs:label xml:lang="en">TaskExecution - end date</rdfs:label>
		  <rdfs:comment xml:lang="en">This property denotes the end time of a TaskExecution.</rdfs:comment>
	 </owl:DatatypeProperty>

<!-- TaskExecution - tags -->
    <owl:ObjectProperty rdf:about="http://stelar-project.eu/klms#hasTags">
		<vann:usageNote xml:lang="en">Optional property. This property links a TaskExecution with one or more tags, each represented as a key/value pair.</vann:usageNote>
		<dct:identifier>klms:hasTags</dct:identifier>
		<rdfs:label xml:lang="en">TaskExecution - hasTags</rdfs:label>
        <rdfs:domain rdf:resource="http://stelar-project.eu/klms#TaskExecution"/>
        <rdfs:range rdf:resource="http://stelar-project.eu/klms#KeyValuePair"/>
        <rdfs:comment xml:lang="en">A tag associated with a TaskExecution and represented as key/value pair.</rdfs:comment>
    </owl:ObjectProperty>
 
<!-- TaskExecution - parameters -->
    <owl:ObjectProperty rdf:about="http://stelar-project.eu/klms#hasParameters">
		<vann:usageNote xml:lang="en">Optional property. This property links a TaskExecution with one or more parameters, each represented as a key/value pair.</vann:usageNote>
		<dct:identifier>klms:hasParameters</dct:identifier>
		<rdfs:label xml:lang="en">TaskExecution - hasParameters</rdfs:label>
        <rdfs:domain rdf:resource="http://stelar-project.eu/klms#TaskExecution"/>
        <rdfs:range rdf:resource="http://stelar-project.eu/klms#KeyValuePair"/>
        <rdfs:comment xml:lang="en">A parameter specification for a TaskExecution, represented as key/value pair.</rdfs:comment>
    </owl:ObjectProperty>
	
<!-- TaskExecution - metrics -->
    <owl:ObjectProperty rdf:about="http://stelar-project.eu/klms#hasMetrics">
		<vann:usageNote xml:lang="en">Optional property. This property links a TaskExecution with one or more metrics (e.g., precision, recall, RMSE, time), each represented as a key/value pair.</vann:usageNote>
		<dct:identifier>klms:hasMetrics</dct:identifier>
		<rdfs:label xml:lang="en">TaskExecution - hasMetrics</rdfs:label>
        <rdfs:domain rdf:resource="http://stelar-project.eu/klms#TaskExecution"/>
        <rdfs:range rdf:resource="http://stelar-project.eu/klms#KeyValuePair"/>
        <rdfs:comment xml:lang="en">A metric associated with a TaskExecution and represented as key/value pair.</rdfs:comment>
    </owl:ObjectProperty>	

<!-- TaskExecution - input -->
    <owl:ObjectProperty rdf:about="http://stelar-project.eu/klms#hasInput">
		<vann:usageNote xml:lang="en">Optional property. This property links a TaskExecution with one or more Distributions used as its input.</vann:usageNote>
		<dct:identifier>klms:hasInput</dct:identifier>
		<rdfs:label xml:lang="en">TaskExecution - hasInput</rdfs:label>
        <rdfs:domain rdf:resource="http://stelar-project.eu/klms#TaskExecution"/>
        <rdfs:range rdf:resource="http://stelar-project.eu/klms#Distribution"/>
        <rdfs:comment xml:lang="en">This property links a TaskExecution with one or more Distributions used as its input.</rdfs:comment>
    </owl:ObjectProperty>

<!-- TaskExecution - output -->
    <owl:ObjectProperty rdf:about="http://stelar-project.eu/klms#hasOutput">
		<vann:usageNote xml:lang="en">Optional property. This property links a TaskExecution with one or more output Distributions (i.e., datasets derived by this execution).</vann:usageNote>
		<dct:identifier>klms:hasOutput</dct:identifier>
		<rdfs:label xml:lang="en">TaskExecution - hasOutput</rdfs:label>
        <rdfs:domain rdf:resource="http://stelar-project.eu/klms#TaskExecution"/>
        <rdfs:range rdf:resource="http://stelar-project.eu/klms#Distribution"/>
        <rdfs:comment xml:lang="en">This property links a TaskExecution with one or more output Distributions (i.e., datasets derived by this execution).</rdfs:comment>
    </owl:ObjectProperty>

 <!--  TaskExecution - creator  -->
	 <owl:ObjectProperty rdf:about="http://purl.org/dc/terms/creator"> 
		  <vann:usageNote xml:lang="en">Optional property. This property refers to the User that triggered this TaskExecution instance.</vann:usageNote>
		  <dct:identifier>dct:creator</dct:identifier>
		  <rdfs:domain rdf:resource="http://stelar-project.eu/klms#TaskExecution"/>
		  <rdfs:range rdf:resource="http://stelar-project.eu/klms#User"/>
		  <rdfs:label xml:lang="en">TaskExecution - creator</rdfs:label>
		  <rdfs:comment xml:lang="en">This property refers to the User that triggered this TaskExecution instance.</rdfs:comment>
	 </owl:ObjectProperty>
	 
<!-- Generated by the OWL API (version 4.2.8.20170104-2310) https://github.com/owlcs/owlapi -->

</rdf:RDF>